@prefix : <http://lei.info/voc/> .
@prefix L1: <http://lei.info/voc/l1/> .
@prefix L2: <http://lei.info/voc/l2/> .
@prefix rr: <http://www.gleif.org/data/schema/rr/2016/> .
@prefix owl: <http://www.w3.org/2002/07/owl#> .
@prefix rdf: <http://www.w3.org/1999/02/22-rdf-syntax-ns#> .
@prefix xml: <http://www.w3.org/XML/1998/namespace> .
@prefix xsd: <http://www.w3.org/2001/XMLSchema#> .
@prefix rdfs: <http://www.w3.org/2000/01/rdf-schema#> .
@base <http://lei.info/voc/> .

<http://lei.info/voc/> rdf:type owl:Ontology ;
                        owl:versionIRI <http://lei.info/voc/> ;
                        rdfs:comment """Contact
Robert Trypuz (robert.trypuz@makolab.com)"""@en ,
                                     """Global Legal Entity Identifier Ontology (GLEIO) for CDF format of LEVEL 1 & 2.

This ontology - Global Legal Entity Identifier Ontology (GLEIO in short) - has been created by MakoLab's R&D Group. GLEIO is a semantic representation of LEI Common Data File format for LEVEL 1 and 2."""@en ;
                        owl:versionInfo "version 1.0"@en .

#################################################################
#    Annotation properties
#################################################################

###  http://lei.info/voc/l1/level1CDFFName
L1:level1CDFFName rdf:type owl:AnnotationProperty ;
                  rdfs:label "level 1 CDF file name"@en .


###  http://lei.info/voc/l1/level1CDFFType
L1:level1CDFFType rdf:type owl:AnnotationProperty ;
                  rdfs:label "level 1 CDF file type name"@en .


###  http://lei.info/voc/l2/level2CDFFName
L2:level2CDFFName rdf:type owl:AnnotationProperty ;
                  rdfs:label "level 2 CDF file name"@en .


###  http://lei.info/voc/l2/level2CDFFType
L2:level2CDFFType rdf:type owl:AnnotationProperty ;
                  rdfs:label "level 2 CDF file type name"@en .


###  http://www.w3.org/2002/07/owl#maxQualifiedCardinality
owl:maxQualifiedCardinality rdf:type owl:AnnotationProperty .


###  http://www.w3.org/2002/07/owl#minQualifiedCardinality
owl:minQualifiedCardinality rdf:type owl:AnnotationProperty .


###  http://www.w3.org/2002/07/owl#qualifiedCardinality
owl:qualifiedCardinality rdf:type owl:AnnotationProperty .


###  http://www.w3.org/2004/02/skos/core#closeMatch
<http://www.w3.org/2004/02/skos/core#closeMatch> rdf:type owl:AnnotationProperty .


###  http://www.w3.org/2004/02/skos/core#definition
<http://www.w3.org/2004/02/skos/core#definition> rdf:type owl:AnnotationProperty .


###  http://www.w3.org/2004/02/skos/core#exactMatch
<http://www.w3.org/2004/02/skos/core#exactMatch> rdf:type owl:AnnotationProperty .


#################################################################
#    Object Properties
#################################################################

###  http://lei.info/voc/l1/address
L1:address rdf:type owl:ObjectProperty ;
           rdfs:subPropertyOf owl:topObjectProperty ;
           rdfs:domain L1:LegalEntity ;
           rdfs:range L1:Address ;
           L1:level1CDFFType "lei:AddressType"^^xsd:string ;
           rdfs:label "has address"@en ;
           <http://www.w3.org/2004/02/skos/core#definition> "An address of the legal entity"@en .


###  http://lei.info/voc/l1/alternativeLanguageHeadquartersAddress
L1:alternativeLanguageHeadquartersAddress rdf:type owl:ObjectProperty ;
                                          rdfs:subPropertyOf L1:address ;
                                          L1:level1CDFFName "ALTERNATIVE_LANGUAGE_HEADQUARTERS_ADDRESS"^^xsd:string ,
                                                            "AddressTypeEnum"^^xsd:string ,
                                                            "OtherAddress"^^xsd:string ,
                                                            "OtherAddresses"^^xsd:string ;
                                          L1:level1CDFFType "lei:AddressTypeEnum"^^xsd:string ,
                                                            "lei:OtherAddressType"^^xsd:string ,
                                                            "lei:OtherAddressesType"^^xsd:string ;
                                          rdfs:label "has alternative language headquarters address"@en ;
                                          <http://www.w3.org/2004/02/skos/core#definition> "Address of the headquarters of the entity in the legal jurisdiction, in an alternative language used in the legal jurisdiction."@en .


###  http://lei.info/voc/l1/alternativeLanguageLegalAddress
L1:alternativeLanguageLegalAddress rdf:type owl:ObjectProperty ;
                                   rdfs:subPropertyOf L1:address ;
                                   L1:level1CDFFName "ALTERNATIVE_LANGUAGE_LEGAL_ADDRESS"^^xsd:string ,
                                                     "AddressTypeEnum"^^xsd:string ,
                                                     "OtherAddress"^^xsd:string ,
                                                     "OtherAddresses"^^xsd:string ;
                                   L1:level1CDFFType "lei:AddressTypeEnum"^^xsd:string ,
                                                     "lei:OtherAddressType"^^xsd:string ,
                                                     "lei:OtherAddressesType"^^xsd:string ;
                                   rdfs:label "has alternative language legal address"@en ;
                                   <http://www.w3.org/2004/02/skos/core#definition> "Registered address of the entity in the legal jurisdiction, in an alternative language used in the legal jurisdiction."@en .


###  http://lei.info/voc/l1/associatedEntityWithLEI
L1:associatedEntityWithLEI rdf:type owl:ObjectProperty ;
                           rdfs:subPropertyOf owl:topObjectProperty ;
                           rdf:type owl:FunctionalProperty ;
                           rdfs:domain L1:LegalEntity ;
                           rdfs:range L1:LegalEntity ;
                           L1:level1CDFFName "AssociatedEntity"^^xsd:string ,
                                             "AssociatedLEI"^^xsd:string ;
                           L1:level1CDFFType "lei:AssociatedEntityType"^^xsd:string ,
                                             "lei:LEIType"^^xsd:string ;
                           rdfs:comment "It is used instead of hasAssociatedEntityWithoutLEI."@en ;
                           rdfs:label "has associated entity with LEI"@en ;
                           <http://www.w3.org/2004/02/skos/core#definition> "The property assigns the entity with LEI associated with the legal entity of this registration."@en .


###  http://lei.info/voc/l1/autoASCIITransliteratedHeadquartersAddress
L1:autoASCIITransliteratedHeadquartersAddress rdf:type owl:ObjectProperty ;
                                              rdfs:subPropertyOf L1:address ;
                                              L1:level1CDFFName "AUTO_ASCII_TRANSLITERATED_HEADQUARTERS_ADDRESS"^^xsd:string ,
                                                                "TransliteratedAddressTypeEnum"^^xsd:string ,
                                                                "TransliteratedOtherAddress"^^xsd:string ,
                                                                "TransliteratedOtherAddresses"^^xsd:string ;
                                              L1:level1CDFFType "lei:TransliteratedAddressTypeEnum"^^xsd:string ,
                                                                "lei:TransliteratedOtherAddressType"^^xsd:string ,
                                                                "lei:TransliteratedOtherAddressesType"^^xsd:string ;
                                              rdfs:label "has auto ASCII transliterated headquarters address"@en ;
                                              <http://www.w3.org/2004/02/skos/core#definition> "Address of the headquarters of the entity, transliterated to ASCII characters, autotransliterated by the managing LOU."@en .


###  http://lei.info/voc/l1/autoASCIITransliteratedLegalAddress
L1:autoASCIITransliteratedLegalAddress rdf:type owl:ObjectProperty ;
                                       rdfs:subPropertyOf L1:address ;
                                       L1:level1CDFFName "AUTO_ASCII_TRANSLITERATED_LEGAL_ADDRESS"^^xsd:string ,
                                                         "TransliteratedAddressTypeEnum"^^xsd:string ,
                                                         "TransliteratedOtherAddress"^^xsd:string ,
                                                         "TransliteratedOtherAddresses"^^xsd:string ;
                                       L1:level1CDFFType "lei:TransliteratedAddressTypeEnum"^^xsd:string ,
                                                         "lei:TransliteratedOtherAddressType"^^xsd:string ,
                                                         "lei:TransliteratedOtherAddressesType"^^xsd:string ;
                                       rdfs:label "has auto ASCII transliterated legal address"@en ;
                                       <http://www.w3.org/2004/02/skos/core#definition> "Registered address of the entity in the legal jurisdiction, transliterated to ASCII characters, autotransliterated by the managing LOU."@en .


###  http://lei.info/voc/l1/entityCategory
L1:entityCategory rdf:type owl:ObjectProperty ,
                           owl:FunctionalProperty ;
                  rdfs:domain L1:LegalEntity ;
                  rdfs:range L1:EntityCategory ;
                  L1:level1CDFFType "EntityCategory"^^xsd:string ;
                  rdfs:label "has legal entity category"@en ;
                  <http://www.w3.org/2004/02/skos/core#definition> "Assigns to a legal entity its category. These categories are based on use cases specified in LEI-ROC policies, found at http://www.leiroc.org/list/leiroc_gls/index.htm (LEI-CDF V2.0)"@en .


###  http://lei.info/voc/l1/entityExpirationReason
L1:entityExpirationReason rdf:type owl:ObjectProperty ,
                                   owl:FunctionalProperty ;
                          rdfs:domain L1:LegalEntity ;
                          rdfs:range L1:EntityExpirationReason ;
                          L1:level1CDFFName "EntityExpirationReason"^^xsd:string ;
                          L1:level1CDFFType "lei:EntityExpirationReasonEnum"^^xsd:string ;
                          rdfs:comment """This element shall be present if entity expiration date is assigned by means of hasEntityExpirationDate datatype property to LE, and omitted otherwise.

See also hasEntityExpirationDate datatype property."""@en ;
                          rdfs:label "has entity expiration reason"@en ;
                          <http://www.w3.org/2004/02/skos/core#definition> "The property assigns to legal entity the reason that it ceased to exist and/or operate."@en .


###  http://lei.info/voc/l1/fundFamily
L1:fundFamily rdf:type owl:ObjectProperty ;
              rdfs:subPropertyOf L1:associatedEntityWithLEI ;
              L1:level1CDFFName "FUND_FAMILY"^^xsd:string ;
              L1:level1CDFFType "lei:AssociatedEntityTypeEnum"^^xsd:string ;
              rdfs:label "has fund family"@en ;
              <http://www.w3.org/2004/02/skos/core#definition> "The legal entity is a fund, and the associated entity is the manager of the fund."@en .


###  http://lei.info/voc/l1/headquartersAddress
L1:headquartersAddress rdf:type owl:ObjectProperty ;
                       rdfs:subPropertyOf L1:address ;
                       rdf:type owl:FunctionalProperty ;
                       L1:level1CDFFName "HeadquartersAddress"^^xsd:string ;
                       L1:level1CDFFType "lei:AddressType"^^xsd:string ;
                       rdfs:label "has headquarters address"@en ;
                       <http://www.w3.org/2004/02/skos/core#definition> "The address of the headquarters of the legal entity."@en .


###  http://lei.info/voc/l1/identifiedBy
L1:identifiedBy rdf:type owl:ObjectProperty ;
                owl:inverseOf L1:identifies ;
                rdf:type owl:FunctionalProperty ,
                         owl:InverseFunctionalProperty ;
                rdfs:domain L1:LegalEntity ;
                rdfs:range L1:LegalEntityIdentifier ;
                L1:level1CDFFName "LEI"^^xsd:string ;
                L1:level1CDFFType "lei:LEIType"^^xsd:string ;
                rdfs:label "is identified by"@en ;
                <http://www.w3.org/2004/02/skos/core#definition> "The property used to assign legal entity identifiers to legal entities."@en .


###  http://lei.info/voc/l1/identifies
L1:identifies rdf:type owl:ObjectProperty ,
                       owl:FunctionalProperty ,
                       owl:InverseFunctionalProperty ;
              rdfs:domain L1:LegalEntityIdentifier ;
              rdfs:range L1:LegalEntity ;
              L1:level1CDFFName "LEI"^^xsd:string ;
              L1:level1CDFFType "lei:LEIType"^^xsd:string ;
              rdfs:label "identifies"@en ;
              <http://www.w3.org/2004/02/skos/core#definition> "The property assigns a (business or global) legal entity identifier to a legal entity."@en .


###  http://lei.info/voc/l1/legalAddress
L1:legalAddress rdf:type owl:ObjectProperty ;
                rdfs:subPropertyOf L1:address ;
                rdf:type owl:FunctionalProperty ;
                L1:level1CDFFName "LegalAddress"^^xsd:string ;
                L1:level1CDFFType "lei:AddressType"^^xsd:string ;
                rdfs:label "has legal address"@en ;
                <http://www.w3.org/2004/02/skos/core#definition> "The address of legal formation of the legal entity as recorded in the registration of the entity in its legal jurisdiction."@en .


###  http://lei.info/voc/l1/legalEntityStatus
L1:legalEntityStatus rdf:type owl:ObjectProperty ,
                              owl:FunctionalProperty ;
                     rdfs:domain L1:LegalEntity ;
                     rdfs:range L1:EntityStatus ;
                     L1:level1CDFFType "EntityStatus"^^xsd:string ;
                     rdfs:label "has status"@en ;
                     <http://www.w3.org/2004/02/skos/core#definition> "The property assigns the status (from the class LegalEntityStatus) to legal entity."@en .


###  http://lei.info/voc/l1/managingLOU
L1:managingLOU rdf:type owl:ObjectProperty ,
                        owl:FunctionalProperty ;
               rdfs:domain L1:LegalEntityIdentifier ;
               L1:level1CDFFName "ManagingLOU"^^xsd:string ;
               L1:level1CDFFType "lei:LEIType"^^xsd:string ;
               rdfs:label "has managing LOU"@en ;
               <http://www.w3.org/2004/02/skos/core#definition> "The LOU that is responsible for administering this LEI registration."@en .


###  http://lei.info/voc/l1/otherValidationAuthority
L1:otherValidationAuthority rdf:type owl:ObjectProperty ;
                            rdfs:domain L1:LegalEntity ;
                            rdfs:range L1:ValidationAuthority ;
                            L1:level1CDFFName "OtherValidationAuthorities"^^xsd:string ,
                                              "OtherValidationAuthority"^^xsd:string ;
                            L1:level1CDFFType "lei:OtherValidationAuthoritiesType"^^xsd:string ,
                                              "lei:OtherValidationAuthorityType"^^xsd:string ;
                            rdfs:label "has other validation authority"@en ;
                            <http://www.w3.org/2004/02/skos/core#definition> "An additional registration authority used by the LOU to validate the entity data."@en .


###  http://lei.info/voc/l1/preferredASCIITransliteratedHeadquartersAddress
L1:preferredASCIITransliteratedHeadquartersAddress rdf:type owl:ObjectProperty ;
                                                   rdfs:subPropertyOf L1:address ;
                                                   L1:level1CDFFName "PREFERRED_ASCII_TRANSLITERATED_HEADQUARTERS_ADDRESS"^^xsd:string ,
                                                                     "TransliteratedAddressTypeEnum"^^xsd:string ,
                                                                     "TransliteratedOtherAddress"^^xsd:string ,
                                                                     "TransliteratedOtherAddresses"^^xsd:string ;
                                                   L1:level1CDFFType "lei:TransliteratedAddressTypeEnum"^^xsd:string ,
                                                                     "lei:TransliteratedOtherAddressType"^^xsd:string ,
                                                                     "lei:TransliteratedOtherAddressesType"^^xsd:string ;
                                                   rdfs:label "has preferred ASCII transliterated headquarters address"@en ;
                                                   <http://www.w3.org/2004/02/skos/core#definition> "Registered address of the entity in the legal jurisdiction, transliterated to ASCII characters, provided by the entity for this purpose."@en .


###  http://lei.info/voc/l1/preferredASCIITransliteratedLegalAddress
L1:preferredASCIITransliteratedLegalAddress rdf:type owl:ObjectProperty ;
                                            rdfs:subPropertyOf L1:address ;
                                            L1:level1CDFFName "PREFERRED_ASCII_TRANSLITERATED_LEGAL_ADDRESS"^^xsd:string ,
                                                              "TransliteratedAddressTypeEnum"^^xsd:string ,
                                                              "TransliteratedOtherAddress"^^xsd:string ,
                                                              "TransliteratedOtherAddresses"^^xsd:string ;
                                            L1:level1CDFFType "lei:TransliteratedAddressTypeEnum"^^xsd:string ,
                                                              "lei:TransliteratedOtherAddressType"^^xsd:string ,
                                                              "lei:TransliteratedOtherAddressesType"^^xsd:string ;
                                            rdfs:label "has preferred ASCII transliterated legal address"@en ;
                                            <http://www.w3.org/2004/02/skos/core#definition> "Registered address of the entity in the legal jurisdiction, transliterated to ASCII characters, provided by the entity for this purpose."@en .


###  http://lei.info/voc/l1/primaryValidationAuthority
L1:primaryValidationAuthority rdf:type owl:ObjectProperty ,
                                       owl:FunctionalProperty ;
                              rdfs:domain L1:LegalEntity ;
                              rdfs:range L1:ValidationAuthority ;
                              L1:level1CDFFType "ValidationAuthorityType"^^xsd:string ;
                              rdfs:label "has primary validation authority"@en ;
                              <http://www.w3.org/2004/02/skos/core#definition> "The (primary) registration authority used by the LOU to validate GLEI data."@en .


###  http://lei.info/voc/l1/registrationAuthority
L1:registrationAuthority rdf:type owl:ObjectProperty ;
                         rdfs:domain L1:LegalEntity ;
                         L1:level1CDFFType "RegistrationAuthorityType"^^xsd:string ;
                         rdfs:label "has registration authority"@en ;
                         <http://www.w3.org/2004/02/skos/core#definition> "A registration authority"@en .


###  http://lei.info/voc/l1/registrationStatus
L1:registrationStatus rdf:type owl:ObjectProperty ,
                               owl:FunctionalProperty ;
                      rdfs:domain L1:LegalEntityIdentifier ;
                      rdfs:range L1:RegistrationStatus ;
                      L1:level1CDFFName "RegistrationStatus"^^xsd:string ;
                      L1:level1CDFFType "lei:RegistrationStatusEnum"^^xsd:string ;
                      rdfs:comment """This is not to be confused with the status of the legal entity itself; see hasEntityStatus.

See also RegistrationStatus class."""@en ;
                      rdfs:label "has registration status"@en ;
                      <http://www.w3.org/2004/02/skos/core#definition> "The status of the legal entity's LEI registration with the Managing LOU."@en .


###  http://lei.info/voc/l1/successorEntityWithLEI
L1:successorEntityWithLEI rdf:type owl:ObjectProperty ,
                                   owl:FunctionalProperty ;
                          rdfs:domain L1:LegalEntity ;
                          rdfs:range L1:LegalEntity ;
                          L1:level1CDFFName "SuccessorEntity"^^xsd:string ,
                                            "SuccessorLEI"^^xsd:string ;
                          L1:level1CDFFType "lei:LEIType"^^xsd:string ,
                                            "lei:SuccessorEntityType"^^xsd:string ;
                          rdfs:label "has successor entity with LEI"@en ;
                          <http://www.w3.org/2004/02/skos/core#definition> """The surviving/new legal entity which continues/replaces this registration. 

The successor entity should have LEI."""@en .


###  http://lei.info/voc/l1/validationSource
L1:validationSource rdf:type owl:ObjectProperty ,
                             owl:FunctionalProperty ;
                    rdfs:domain L1:LegalEntity ;
                    rdfs:range L1:ValidationSource ;
                    L1:level1CDFFType "ValidationSources"^^xsd:string ;
                    rdfs:comment "It is omitted if the validation status is not known or not revealed."@en ;
                    rdfs:label "has validation source"@en ;
                    <http://www.w3.org/2004/02/skos/core#definition> "The property assigns the current validation status (from ValidationSource class) to this LEI record."@en .


###  http://lei.info/voc/l2/childLegalEntity
L2:childLegalEntity rdf:type owl:ObjectProperty ;
                    rdfs:domain L2:Relationship ;
                    rdfs:range L2:LegalEntity ;
                    L2:level2CDFFName "NodeID"^^xsd:string ,
                                      "StartNode"^^xsd:string ;
                    L2:level2CDFFType "rr:LEIType"^^xsd:string ,
                                      "rr:NodeType"^^xsd:string ;
                    rdfs:label "has child legal entity"@en ;
                    <http://www.w3.org/2004/02/skos/core#definition> "The entity at the \"start\" of a directional relationship."@en .


###  http://lei.info/voc/l2/managingLOU
L2:managingLOU rdf:type owl:ObjectProperty ;
               rdfs:domain L2:Relationship ;
               rdfs:range L2:LocalOperatingUnit ;
               L2:level2CDFFName "ManagingLOU"^^xsd:string ;
               L2:level2CDFFType "rr:LEIType"^^xsd:string ;
               rdfs:label "has managing LOU"@en ;
               <http://www.w3.org/2004/02/skos/core#definition> "The LOU that is responsible for administering this relationship record."@en .


###  http://lei.info/voc/l2/measurementMethod
L2:measurementMethod rdf:type owl:ObjectProperty ;
                     rdfs:domain L2:RelationshipQuantifier ;
                     rdfs:range L2:MeasurementMethod ;
                     L2:level2CDFFName "MeasurementMethod"^^xsd:string ;
                     L2:level2CDFFType "rr:RelationshipQuantifierType"^^xsd:string ;
                     rdfs:label "has measurement method"@en ;
                     <http://www.w3.org/2004/02/skos/core#definition> "This property specifies the method of measurement (or set of rules) used to quantitatively categorize the relationship."@en .


###  http://lei.info/voc/l2/parentLegalEntity
L2:parentLegalEntity rdf:type owl:ObjectProperty ;
                     rdfs:domain L2:Relationship ;
                     rdfs:range L2:LegalEntity ;
                     L2:level2CDFFName "EndNode"^^xsd:string ,
                                       "NodeID"^^xsd:string ;
                     L2:level2CDFFType "rr:LEIType"^^xsd:string ,
                                       "rr:NodeType"^^xsd:string ;
                     rdfs:label "has parent legal entity"@en ;
                     <http://www.w3.org/2004/02/skos/core#definition> "The entity at the \"end\" of a directional relationship."@en .


###  http://lei.info/voc/l2/qualifierCategory
L2:qualifierCategory rdf:type owl:ObjectProperty ;
                     rdfs:domain L2:RelationshipQualifier ;
                     rdfs:range L2:RelationshipQualifierCategory ;
                     L2:level2CDFFName "QualifierCategory"^^xsd:string ;
                     L2:level2CDFFType "rr:QualifierCategoryTypeEnum"^^xsd:string ;
                     rdfs:label "has qualifier category"@en ;
                     <http://www.w3.org/2004/02/skos/core#definition> "This property specifies the additional qualitative attributes that help to categorize the relationship."@en .


###  http://lei.info/voc/l2/qualifierDimension
L2:qualifierDimension rdf:type owl:ObjectProperty ;
                      rdfs:domain L2:RelationshipQualifier ;
                      rdfs:range L2:RelationshipQualifierDimension ;
                      L2:level2CDFFName "QualifierDimension"^^xsd:string ;
                      L2:level2CDFFType "rr:QualifierDimensionEnum"^^xsd:string ;
                      rdfs:label "has qualifier dimension"@en ;
                      <http://www.w3.org/2004/02/skos/core#definition> "This property designates the optional list of additional qualitative attributes that help to categorize the relationship."@en .


###  http://lei.info/voc/l2/quantifierUnit
L2:quantifierUnit rdf:type owl:ObjectProperty ;
                  rdfs:domain L2:RelationshipQuantifier ;
                  rdfs:range L2:RelationshipQuantifierUnit ;
                  L2:level2CDFFName "QuantifierUnits"^^xsd:string ;
                  L2:level2CDFFType "rr:QuantifierUnitsTypeEnum"^^xsd:string ;
                  rdfs:comment "enumeration PERCENTAGE"@en ;
                  rdfs:label "has quantifier unit"@en ;
                  <http://www.w3.org/2004/02/skos/core#definition> "This property specifies the units, where applicable, of a measurement made on a relationship."@en .


###  http://lei.info/voc/l2/registrationStatus
L2:registrationStatus rdf:type owl:ObjectProperty ;
                      rdfs:domain L2:Relationship ;
                      rdfs:range L2:RegistrationStatus ;
                      L2:level2CDFFName "RegistrationStatus"^^xsd:string ;
                      L2:level2CDFFType "rr:RegistrationStatusEnum"^^xsd:string ;
                      rdfs:comment """This is not to be confused with the status of the relationship itself; see hasRelationshipStatus.

See also RegistrationStatus class."""@en ;
                      rdfs:label "has registration status"@en ;
                      <http://www.w3.org/2004/02/skos/core#definition> "The status of the legal entity's relationship record registration with the managing LOU."@en .


###  http://lei.info/voc/l2/relationshipPeriod
L2:relationshipPeriod rdf:type owl:ObjectProperty ;
                      rdfs:domain L2:Relationship ;
                      rdfs:range [ rdf:type owl:Class ;
                                   owl:unionOf ( L2:AccountingPeriod
                                                 L2:DocumentFilingPeriod
                                                 L2:RelationshipPeriod
                                               )
                                 ] ;
                      L2:level2CDFFName "RelationshipPeriod"^^xsd:string ;
                      L2:level2CDFFType "rr:RelationshipPeriodType"^^xsd:string ;
                      rdfs:label "has relationship period"@en ;
                      <http://www.w3.org/2004/02/skos/core#definition> "This property assigns one set of start and end dates for a particular type of period, for example, the duration of the relationship itself, the filing or validity period of any documents demonstrating the relationship, or the accounting period they refer to."@en .


###  http://lei.info/voc/l2/relationshipQualifier
L2:relationshipQualifier rdf:type owl:ObjectProperty ;
                         rdfs:domain L2:Relationship ;
                         rdfs:range L2:RelationshipQualifier ;
                         L2:level2CDFFName "RelationshipQualifier"^^xsd:string ;
                         L2:level2CDFFType "rr:RelationshipQualifierType"^^xsd:string ;
                         rdfs:label "has relationship qualifier"@en ;
                         <http://www.w3.org/2004/02/skos/core#definition> "This property specifies relationship qualifier information."@en .


###  http://lei.info/voc/l2/relationshipQuantifier
L2:relationshipQuantifier rdf:type owl:ObjectProperty ;
                          rdfs:domain L2:Relationship ;
                          rdfs:range L2:RelationshipQuantifier ;
                          L2:level2CDFFName "RelationshipQuantifier"^^xsd:string ;
                          L2:level2CDFFType "rr:RelationshipQuantifierType"^^xsd:string ;
                          rdfs:label "has relationship quantifier"@en ;
                          <http://www.w3.org/2004/02/skos/core#definition> "This property specifies any additional quantitative attributes that help to categorize the relationship."@en .


###  http://lei.info/voc/l2/relationshipStatus
L2:relationshipStatus rdf:type owl:ObjectProperty ;
                      rdfs:domain L2:Relationship ;
                      rdfs:range L2:RelationshipStatus ;
                      L2:level2CDFFName "RelationshipStatus"^^xsd:string ;
                      L2:level2CDFFType "rr:RelationshipStatusEnum"^^xsd:string ;
                      rdfs:label "has relationship status"@en ;
                      <http://www.w3.org/2004/02/skos/core#definition> "This property assigns the status of the legal entities' relationship itself: ACTIVE or INACTIVE."@en .


###  http://lei.info/voc/l2/relationshipType
L2:relationshipType rdf:type owl:ObjectProperty ;
                    rdfs:domain L2:Relationship ;
                    rdfs:range L2:RelationshipType ;
                    L2:level2CDFFName "RelationshipType"^^xsd:string ;
                    L2:level2CDFFType "rr:RelationshipTypeEnum"^^xsd:string ;
                    rdfs:label "has relationship type"@en ;
                    <http://www.w3.org/2004/02/skos/core#definition> "This property assigns a unique code designating the specific category of a directional relationship between two legal entities."@en .


###  http://lei.info/voc/l2/validationDocument
L2:validationDocument rdf:type owl:ObjectProperty ;
                      rdfs:domain L2:Relationship ;
                      rdfs:range L2:ValidationDocument ;
                      L2:level2CDFFName "ValidationDocuments"^^xsd:string ;
                      L2:level2CDFFType "rr:ValidationDocumentsTypeEnum"^^xsd:string ;
                      rdfs:label "has relationship validation document type"@en ;
                      <http://www.w3.org/2004/02/skos/core#definition> "This property assigns a type of source document(s) used for validating the relationship."@en .


#################################################################
#    Data properties
#################################################################

###  http://lei.info/voc/l1/addressDescriptionComponent
L1:addressDescriptionComponent rdf:type owl:DatatypeProperty ;
                               rdfs:label "address description component"@en ;
                               <http://www.w3.org/2004/02/skos/core#definition> "address description component"@en .


###  http://lei.info/voc/l1/addressNumber
L1:addressNumber rdf:type owl:DatatypeProperty ;
                 rdfs:subPropertyOf L1:addressDescriptionComponent ;
                 rdf:type owl:FunctionalProperty ;
                 rdfs:domain L1:Address ;
                 rdfs:range [ rdf:type rdfs:Datatype ;
                              owl:unionOf ( rdf:PlainLiteral
                                            xsd:string
                                          )
                            ] ;
                 L1:level1CDFFType "AddressNumber"^^xsd:string ,
                                   "lei:Tokenized500Type"^^xsd:string ;
                 rdfs:comment """An element of this type has minimum length of one character and may not contain any of: the carriage return (#xD), line feed (#xA) nor tab (#x9) characters, shall not begin or end with a space (#x20) character, or a sequence of two or more adjacent space characters.

restriction of xs:string
minLength 1
maxLength 500
pattern \\\\S+( \\\\S+)*"""@en ;
                 rdfs:label "has address number"@en ;
                 <http://www.w3.org/2004/02/skos/core#definition> "Optional, additional structured version of an external house number, or range of numbers, contained in one of the address line elements. This could be a numeral, a letter or code made up of mixed characters (e.g. 221B)."@en .


###  http://lei.info/voc/l1/addressNumberWithinBuilding
L1:addressNumberWithinBuilding rdf:type owl:DatatypeProperty ;
                               rdfs:subPropertyOf L1:addressDescriptionComponent ;
                               rdf:type owl:FunctionalProperty ;
                               rdfs:domain L1:Address ;
                               rdfs:range [ rdf:type rdfs:Datatype ;
                                            owl:unionOf ( rdf:PlainLiteral
                                                          xsd:string
                                                        )
                                          ] ;
                               L1:level1CDFFName "AddressNumberWithinBuilding"^^xsd:string ;
                               L1:level1CDFFType "lei:Tokenized500Type"^^xsd:string ;
                               rdfs:comment """An element of this type has minimum length of one character and may not contain any of: the carriage return (#xD), line feed (#xA) nor tab (#x9) characters, shall not begin or end with a space (#x20) character, or a sequence of two or more adjacent space characters.

restriction of xs:string
minLength 1
maxLength 500
pattern \\\\S+( \\\\S+)*"""@en ;
                               rdfs:label "has address number with building"@en ;
                               <http://www.w3.org/2004/02/skos/core#definition> "Optional, additional structured version of an internal location number, or range of numbers, contained in one of the address line elements.This could be a numeral, a letter or code made up of mixed characters (e.g. 13) of a floor, suite or apartment within a building identified e.g. by an AddressNumber element."@en .


###  http://lei.info/voc/l1/alternativeLanguageEntityName
L1:alternativeLanguageEntityName rdf:type owl:DatatypeProperty ;
                                 rdfs:subPropertyOf L1:otherEntityName ;
                                 rdfs:domain L1:LegalEntity ;
                                 rdfs:range [ rdf:type rdfs:Datatype ;
                                              owl:unionOf ( rdf:PlainLiteral
                                                            xsd:string
                                                          )
                                            ] ;
                                 L1:level1CDFFName "ALTERNATIVE_LANGUAGE_LEGAL_NAME"^^xsd:string ;
                                 L1:level1CDFFType "lei:EntityNameTypeEnum"^^xsd:string ,
                                                   "lei:Tokenized500Type"^^xsd:string ;
                                 rdfs:comment """An element of this type has minimum length of one character and may not contain any of: the carriage return (#xD), line feed (#xA) nor tab (#x9) characters, shall not begin or end with a space (#x20) character, or a sequence of two or more adjacent space characters.

restriction of xs:string
minLength 1
maxLength 500
pattern \\\\S+( \\\\S+)*"""@en ;
                                 rdfs:label "has other entity name"@en ;
                                 <http://www.w3.org/2004/02/skos/core#definition> "Registered name of the entity in an alternative language in the legal jurisdiction in which the entity is registered."@en .


###  http://lei.info/voc/l1/associatedEntityWithoutLEI
L1:associatedEntityWithoutLEI rdf:type owl:DatatypeProperty ;
                              rdfs:subPropertyOf L1:legalEntityDescriptionComponent ;
                              rdf:type owl:FunctionalProperty ;
                              rdfs:domain L1:LegalEntity ;
                              rdfs:range [ rdf:type rdfs:Datatype ;
                                           owl:unionOf ( rdf:PlainLiteral
                                                         xsd:string
                                                       )
                                         ] ;
                              L1:level1CDFFName "AssociatedEntity"^^xsd:string ,
                                                "AssociatedEntityName"^^xsd:string ;
                              L1:level1CDFFType "lei:AssociatedEntityType"^^xsd:string ,
                                                "lei:NameType"^^xsd:string ,
                                                "lei:Tokenized500Type"^^xsd:string ;
                              rdfs:comment "It is used instead of hasAssociatedEntityWithLEI."@en ;
                              rdfs:label "has associated entity without LEI"@en ;
                              <http://www.w3.org/2004/02/skos/core#definition> "The property assigns the name of an entity associated with the legal entity of this registration."@en .


###  http://lei.info/voc/l1/autoASCIITransliteratedLegalName
L1:autoASCIITransliteratedLegalName rdf:type owl:DatatypeProperty ;
                                    rdfs:subPropertyOf L1:transliteratedOtherEntityName ;
                                    rdfs:domain L1:LegalEntity ;
                                    rdfs:range [ rdf:type rdfs:Datatype ;
                                                 owl:unionOf ( rdf:PlainLiteral
                                                               xsd:string
                                                             )
                                               ] ;
                                    L1:level1CDFFName "AUTO_ASCII_TRANSLITERATED_LEGAL_ADDRESS"^^xsd:string ;
                                    L1:level1CDFFType "lei:Tokenized500Type"^^xsd:string ,
                                                      "lei:TransliteratedEntityNameTypeEnum"^^xsd:string ;
                                    rdfs:comment """An element of this type has minimum length of one character and may not contain any of: the carriage return (#xD), line feed (#xA) nor tab (#x9) characters, shall not begin or end with a space (#x20) character, or a sequence of two or more adjacent space characters.

restriction of xs:string
minLength 1
maxLength 500
pattern \\\\S+( \\\\S+)*"""@en ;
                                    rdfs:label "has ASCII-transliterated representation of legal name"@en ;
                                    <http://www.w3.org/2004/02/skos/core#definition> "Legal name of the entity transliterated to ASCII characters, auto-transliterated by the managing LOU."@en .


###  http://lei.info/voc/l1/city
L1:city rdf:type owl:DatatypeProperty ;
        rdfs:subPropertyOf L1:addressDescriptionComponent ;
        rdf:type owl:FunctionalProperty ;
        rdfs:domain L1:Address ;
        rdfs:range [ rdf:type rdfs:Datatype ;
                     owl:unionOf ( rdf:PlainLiteral
                                   xsd:string
                                 )
                   ] ;
        L1:level1CDFFName "City"^^xsd:string ;
        L1:level1CDFFType "lei:Tokenized500Type"^^xsd:string ;
        rdfs:comment """An element of this type has minimum length of one character and may not contain any of: the carriage return (#xD), line feed (#xA) nor tab (#x9) characters, shall not begin or end with a space (#x20) character, or a sequence of two or more adjacent space characters.

restriction of xs:string
minLength 1
maxLength 500
pattern \\\\S+( \\\\S+)*"""@en ;
        rdfs:label "has city"@en ;
        <http://www.w3.org/2004/02/skos/core#definition> "The property assigns to an address of legal entity a name of the city."@en .


###  http://lei.info/voc/l1/country
L1:country rdf:type owl:DatatypeProperty ;
           rdfs:subPropertyOf L1:addressDescriptionComponent ;
           rdf:type owl:FunctionalProperty ;
           rdfs:domain L1:Address ;
           rdfs:range xsd:string ;
           L1:level1CDFFName "Country"^^xsd:string ;
           L1:level1CDFFType "lei:CountryCodeType"^^xsd:string ;
           rdfs:comment """minLength 2 
maxLength 2
pattern ([A-Z]{2})"""@en ;
           rdfs:label "has country code"@en ;
           <http://www.w3.org/2004/02/skos/core#definition> "The property assigns the 2-character ISO 3166-1 country code of the country."@en .


###  http://lei.info/voc/l1/date
L1:date rdf:type owl:DatatypeProperty ;
        rdfs:range xsd:dateTimeStamp ;
        rdfs:label "date"@en ;
        <http://www.w3.org/2004/02/skos/core#definition> "date"@en .


###  http://lei.info/voc/l1/entityExpirationDate
L1:entityExpirationDate rdf:type owl:DatatypeProperty ;
                        rdfs:subPropertyOf L1:date ,
                                           L1:legalEntityDescriptionComponent ;
                        rdf:type owl:FunctionalProperty ;
                        rdfs:domain L1:LegalEntity ;
                        rdfs:range xsd:dateTimeStamp ;
                        L1:level1CDFFName "EntityExpirationDate"^^xsd:string ;
                        L1:level1CDFFType "lei:LEIDateTimeProfile"^^xsd:string ;
                        rdfs:comment """Omitted if LE has not ceased to operate.

If LE ceased to operate (due to dissolution, merger or acquisition), them it is required to point out the expiration reason. Use hasEntityExpirationReason object property."""@en ,
                                     """pattern
([^\\\\.]*|([^\\\\.]*(\\\\.((\\\\d){1,3})){0,1}))(Z|\\\\+([01][0- 9]|2[0-3]):([0-5][0-9])|-([01][0-9]|2[0-3]):([0- 5][0-9]))"""@en ;
                        rdfs:label "has entity expiration date"@en ;
                        <http://www.w3.org/2004/02/skos/core#definition> "The date that the legal entity ceased to operate, whether due to dissolution, merger or acquisition."@en .


###  http://lei.info/voc/l1/entityLegalFormCode
L1:entityLegalFormCode rdf:type owl:DatatypeProperty ;
                       rdfs:subPropertyOf L1:legalEntityDescriptionComponent ;
                       rdf:type owl:FunctionalProperty ;
                       rdfs:domain L1:LegalEntity ;
                       rdfs:range xsd:string ;
                       L1:level1CDFFName "EntityLegalFormCode"^^xsd:string ,
                                         "LegalForm"^^xsd:string ;
                       L1:level1CDFFType "lei:LegalFormEnum"^^xsd:string ,
                                         "lei:LegalFormType"^^xsd:string ;
                       rdfs:comment """pattern 
(([A-Z][A-Z0-9]{3}|[A-Z0-9][A-Z][A-Z0-9]{2}|[A-Z0-9]{2}[A-Z][A-Z0-9]|[A-Z0- 9]{3}[A-Z]))|(9999)|(8888)"""@en ;
                       rdfs:label "has entity legal form"@en ;
                       <http://www.w3.org/2004/02/skos/core#definition> """The legal form of the entity, taken from the ISO Entity Legal Form (ELF) code list maintained by GLEIF.

Please note that the XML schema validates for all Legal Form values conforming to the ISO 20275 standard (section \"Code Structure\"); four uppercase alphanumeric characters in any combination except for purely numeric codes. Some possible combinations may not be valid Entity Legal Form (ELF) entries."""@en .


###  http://lei.info/voc/l1/fundFamilyWithoutLEI
L1:fundFamilyWithoutLEI rdf:type owl:DatatypeProperty ;
                        rdfs:subPropertyOf L1:associatedEntityWithoutLEI ;
                        rdfs:domain L1:LegalEntity ;
                        rdfs:range [ rdf:type rdfs:Datatype ;
                                     owl:unionOf ( rdf:PlainLiteral
                                                   xsd:string
                                                 )
                                   ] ;
                        L1:level1CDFFName "FUND_FAMILY"^^xsd:string ;
                        L1:level1CDFFType "lei:AssociatedEntityTypeEnum"^^xsd:string ,
                                          "lei:Tokenized500Type"^^xsd:string ;
                        rdfs:comment """An element of this type has minimum length of one character and may not contain any of: the carriage return (#xD), line feed (#xA) nor tab (#x9) characters, shall not begin or end with a space (#x20) character, or a sequence of two or more adjacent space characters.

restriction of xs:string
minLength 1
maxLength 500
pattern \\\\S+( \\\\S+)*"""@en ;
                        rdfs:label "has fund family"@en ;
                        <http://www.w3.org/2004/02/skos/core#definition> "The legal entity is a fund, and the associated entity is the manager of the fund."@en .


###  http://lei.info/voc/l1/initialRegistrationDate
L1:initialRegistrationDate rdf:type owl:DatatypeProperty ;
                           rdfs:subPropertyOf L1:date ,
                                              L1:leiDescriptionComponent ;
                           rdf:type owl:FunctionalProperty ;
                           rdfs:domain L1:LegalEntityIdentifier ;
                           rdfs:range xsd:dateTimeStamp ;
                           L1:level1CDFFName "InitialRegistrationDate"^^xsd:string ;
                           L1:level1CDFFType "lei:LEIDateTimeProfile"^^xsd:string ;
                           rdfs:comment """pattern
([^\\\\.]*|([^\\\\.]*(\\\\.((\\\\d){1,3})){0,1}))(Z|\\\\+([01][0- 9]|2[0-3]):([0-5][0-9])|-([01][0-9]|2[0-3]):([0- 5][0-9]))"""@en ;
                           rdfs:label "has initial registration date"@en ;
                           <http://www.w3.org/2004/02/skos/core#definition> "The property assigns date/time the record of general legal entity identifier was created."@en .


###  http://lei.info/voc/l1/lastUpdateDate
L1:lastUpdateDate rdf:type owl:DatatypeProperty ;
                  rdfs:subPropertyOf L1:date ,
                                     L1:leiDescriptionComponent ;
                  rdf:type owl:FunctionalProperty ;
                  rdfs:domain L1:LegalEntityIdentifier ;
                  rdfs:range xsd:dateTimeStamp ;
                  L1:level1CDFFName "LastUpdateDate"^^xsd:string ;
                  L1:level1CDFFType "lei:LEIDateTimeProfile"^^xsd:string ;
                  rdfs:comment """pattern
([^\\\\.]*|([^\\\\.]*(\\\\.((\\\\d){1,3})){0,1}))(Z|\\\\+([01][0- 9]|2[0-3]):([0-5][0-9])|-([01][0-9]|2[0-3]):([0- 5][0-9]))"""@en ;
                  rdfs:label "has last update date"@en ;
                  <http://www.w3.org/2004/02/skos/core#definition> "Date/time the LEI record was most recently updated."@en .


###  http://lei.info/voc/l1/legalEntityDescriptionComponent
L1:legalEntityDescriptionComponent rdf:type owl:DatatypeProperty ;
                                   rdfs:label "legal entity description component"@en ;
                                   <http://www.w3.org/2004/02/skos/core#definition> "legal entity description component"@en .


###  http://lei.info/voc/l1/legalJurisdiction
L1:legalJurisdiction rdf:type owl:DatatypeProperty ;
                     rdfs:subPropertyOf L1:legalEntityDescriptionComponent ;
                     rdf:type owl:FunctionalProperty ;
                     rdfs:domain L1:LegalEntity ;
                     rdfs:range xsd:string ;
                     L1:level1CDFFName "LegalJurisdiction"^^xsd:string ;
                     L1:level1CDFFType "lei:JurisdictionCodeType"^^xsd:string ;
                     rdfs:comment """The property assigns the 2-character ISO 3166-1 country code of the country or the 4- to 6-character ISO 3166-2 region code of the region.

minLength 2 
maxLength 2
pattern ([A-Z]{2})

OR

minLength 4
maxLength 6
pattern ([A-Z]{2}-[A-Z0-9]{1,3})"""@en ;
                     rdfs:label "has jurisdiction of legal formation and registration"@en ;
                     <http://www.w3.org/2004/02/skos/core#definition> "The jurisdiction of legal formation and registration of the entity (and upon which the Legal Form data element is also dependent)."@en .


###  http://lei.info/voc/l1/legalName
L1:legalName rdf:type owl:DatatypeProperty ;
             rdfs:subPropertyOf L1:legalEntityDescriptionComponent ,
                                L1:name ;
             rdf:type owl:FunctionalProperty ;
             rdfs:domain L1:LegalEntity ;
             rdfs:range [ rdf:type rdfs:Datatype ;
                          owl:unionOf ( rdf:PlainLiteral
                                        xsd:string
                                      )
                        ] ;
             L1:level1CDFFName "LegalName"^^xsd:string ;
             L1:level1CDFFType "lei:NameType"^^xsd:string ;
             rdfs:comment """An element of this type has minimum length of one character and may not contain any of: the carriage return (#xD), line feed (#xA) nor tab (#x9) characters, shall not begin or end with a space (#x20) character, or a sequence of two or more adjacent space characters.

restriction of xs:string
minLength 1
maxLength 500
pattern \\\\S+( \\\\S+)*"""@en ;
             rdfs:label "has legal name"@en ;
             <http://www.w3.org/2004/02/skos/core#definition> "The legal name of the entity."@en .


###  http://lei.info/voc/l1/leiCode
L1:leiCode rdf:type owl:DatatypeProperty ;
           rdfs:subPropertyOf L1:leiDescriptionComponent ;
           rdf:type owl:FunctionalProperty ;
           rdfs:domain L1:LegalEntityIdentifier ;
           rdfs:range xsd:string ;
           L1:level1CDFFName "LEI"^^xsd:string ;
           L1:level1CDFFType "LEIType"^^xsd:string ;
           rdfs:comment """minLength 20
maxLength 20
pattern ([0-9A-Z]{18}[0-9]{2})"""@en ;
           rdfs:label "has global legal entity identifier code"@en ;
           <http://www.w3.org/2004/02/skos/core#definition> "Property assigning to the general legal entity identifier a unique 20-character alphanumeric code, defined in the ISO 17442 standard."@en ;
           <http://www.w3.org/2004/02/skos/core#exactMatch> "http://schema.org/leiCode"^^xsd:anyURI .


###  http://lei.info/voc/l1/leiDescriptionComponent
L1:leiDescriptionComponent rdf:type owl:DatatypeProperty ;
                           rdfs:label "LEI description component"@en ;
                           <http://www.w3.org/2004/02/skos/core#definition> "LEI description component"@en .


###  http://lei.info/voc/l1/mailRouting
L1:mailRouting rdf:type owl:DatatypeProperty ;
               rdfs:subPropertyOf L1:addressDescriptionComponent ;
               rdf:type owl:FunctionalProperty ;
               rdfs:domain L1:Address ;
               rdfs:range [ rdf:type rdfs:Datatype ;
                            owl:unionOf ( rdf:PlainLiteral
                                          xsd:string
                                        )
                          ] ;
               L1:level1CDFFType "MailRouting"^^xsd:string ,
                                 "lei:Tokenized500Type"^^xsd:string ;
               rdfs:comment """An element of this type has minimum length of one character and may not contain any of: the carriage return (#xD), line feed (#xA) nor tab (#x9) characters, shall not begin or end with a space (#x20) character, or a sequence of two or more adjacent space characters.

restriction of xs:string
minLength 1
maxLength 500
pattern \\\\S+( \\\\S+)*"""@en ;
               rdfs:label "has mail routing"@en ;
               <http://www.w3.org/2004/02/skos/core#definition> "Optional free text address line to hold content from other address lines containing explicit routing information (this element's presence indicates that this address is a routing address."@en .


###  http://lei.info/voc/l1/name
L1:name rdf:type owl:DatatypeProperty ;
        rdfs:label "name"@en ;
        <http://www.w3.org/2004/02/skos/core#definition> "name"@en .


###  http://lei.info/voc/l1/nextRenewalDate
L1:nextRenewalDate rdf:type owl:DatatypeProperty ;
                   rdfs:subPropertyOf L1:date ,
                                      L1:leiDescriptionComponent ;
                   rdf:type owl:FunctionalProperty ;
                   rdfs:domain L1:LegalEntityIdentifier ;
                   rdfs:range xsd:dateTimeStamp ;
                   L1:level1CDFFName "NextRenewalDate"^^xsd:string ;
                   L1:level1CDFFType "lei:LEIDateTimeProfile"^^xsd:string ;
                   rdfs:comment """pattern
([^\\\\.]*|([^\\\\.]*(\\\\.((\\\\d){1,3})){0,1}))(Z|\\\\+([01][0- 9]|2[0-3]):([0-5][0-9])|-([01][0-9]|2[0-3]):([0- 5][0-9]))"""@en ;
                   rdfs:label "has next renewal date"@en ;
                   <http://www.w3.org/2004/02/skos/core#definition> "The next date by which the LEI registration should be renewed and re-certified by the legal entity."@en .


###  http://lei.info/voc/l1/otherEntityName
L1:otherEntityName rdf:type owl:DatatypeProperty ;
                   rdfs:subPropertyOf L1:legalEntityDescriptionComponent ,
                                      L1:name ;
                   rdfs:domain L1:LegalEntity ;
                   rdfs:range [ rdf:type rdfs:Datatype ;
                                owl:unionOf ( rdf:PlainLiteral
                                              xsd:string
                                            )
                              ] ;
                   L1:level1CDFFName "OtherEntityName"^^xsd:string ,
                                     "OtherEntityNames"^^xsd:string ;
                   L1:level1CDFFType "lei:OtherEntityNameType"^^xsd:string ,
                                     "lei:OtherEntityNamesType"^^xsd:string ;
                   rdfs:label "has other entity name"@en ;
                   <http://www.w3.org/2004/02/skos/core#definition> "An alternative name or representation of a name for the legal entity, excluding transliterations. An optional list of other names."@en .


###  http://lei.info/voc/l1/otherLegalForm
L1:otherLegalForm rdf:type owl:DatatypeProperty ;
                  rdfs:subPropertyOf L1:legalEntityDescriptionComponent ;
                  rdf:type owl:FunctionalProperty ;
                  rdfs:domain L1:LegalEntity ;
                  rdfs:range xsd:string ;
                  L1:level1CDFFName "OtherLegalForm"^^xsd:string ;
                  L1:level1CDFFType "lei:Tokenized500Type"^^xsd:string ;
                  rdfs:comment """An element of this type has minimum length of one character and may not contain any of: the carriage return (#xD), line feed (#xA) nor tab (#x9) characters, shall not begin or end with a space (#x20) character, or a sequence of two or more adjacent space characters.

restriction of xs:string
minLength 1
maxLength 500
pattern \\\\S+( \\\\S+)*"""@en ;
                  rdfs:label "has other legal form"@en ;
                  <http://www.w3.org/2004/02/skos/core#definition> "The property assigns a legacy code or textual description for the legal entity's legal form, used until a current code from the GLEIF-maintained list can be used."@en .


###  http://lei.info/voc/l1/otherRegistrationAuthorityID
L1:otherRegistrationAuthorityID rdf:type owl:DatatypeProperty ;
                                rdfs:subPropertyOf L1:registrationAuthorityDescriptionComponent ;
                                L1:level1CDFFName "OtherRegistrationAuthorityID"^^xsd:string ;
                                L1:level1CDFFType "lei:Tokenized500Type"^^xsd:string ;
                                rdfs:comment """An element of this type has minimum length of one character and may not contain any of: the carriage return (#xD), line feed (#xA) nor tab (#x9) characters, shall not begin or end with a space (#x20) character, or a sequence of two or more adjacent space characters.

restriction of xs:string
minLength 1
maxLength 500
pattern \\\\S+( \\\\S+)*"""@en ;
                                rdfs:label "has other validation authority ID"@en ;
                                <http://www.w3.org/2004/02/skos/core#definition> "A legacy / historical reference code of a registration authority which is not yet entered in the Registration Authorities Code List (RAL) maintained by GLEIF, or the designation of an interim register until such time as an entry from RAL can be delivered."@en .


###  http://lei.info/voc/l1/otherValidationAuthorityID
L1:otherValidationAuthorityID rdf:type owl:DatatypeProperty ;
                              rdfs:subPropertyOf L1:validationAuthorityDescriptionComponent ;
                              rdf:type owl:FunctionalProperty ;
                              rdfs:domain L1:ValidationAuthority ;
                              rdfs:range xsd:string ;
                              L1:level1CDFFName "OtherValidationAuthorityID"^^xsd:string ;
                              L1:level1CDFFType "lei:Tokenized500Type"^^xsd:string ;
                              rdfs:comment """An element of this type has minimum length of one character and may not contain any of: the carriage return (#xD), line feed (#xA) nor tab (#x9) characters, shall not begin or end with a space (#x20) character, or a sequence of two or more adjacent space characters.

restriction of xs:string
minLength 1
maxLength 500
pattern \\\\S+( \\\\S+)*"""@en ;
                              rdfs:label "has other validation authority ID"@en ;
                              <http://www.w3.org/2004/02/skos/core#definition> "A legacy / historical reference code of a registration authority which is not yet entered in the Registration Authorities Code List (RAL) maintained by GLEIF, or the designation of an interim register until such time as an entry from RAL can be delivered."@en .


###  http://lei.info/voc/l1/postalCode
L1:postalCode rdf:type owl:DatatypeProperty ;
              rdfs:subPropertyOf L1:addressDescriptionComponent ;
              rdf:type owl:FunctionalProperty ;
              rdfs:domain L1:Address ;
              rdfs:range [ rdf:type rdfs:Datatype ;
                           owl:unionOf ( rdf:PlainLiteral
                                         xsd:string
                                       )
                         ] ;
              L1:level1CDFFName "PostalCode"^^xsd:string ;
              L1:level1CDFFType "lei:Tokenized500Type"^^xsd:string ;
              rdfs:comment """An element of this type has minimum length of one character and may not contain any of: the carriage return (#xD), line feed (#xA) nor tab (#x9) characters, shall not begin or end with a space (#x20) character, or a sequence of two or more adjacent space characters.

restriction of xs:string
minLength 1
maxLength 500
pattern \\\\S+( \\\\S+)*"""@en ;
              rdfs:label "has postal code"@en ;
              <http://www.w3.org/2004/02/skos/core#definition> "The property assigns the postal code to the address of legal entity."@en .


###  http://lei.info/voc/l1/preferredASCIITransliteratedLegalName
L1:preferredASCIITransliteratedLegalName rdf:type owl:DatatypeProperty ;
                                         rdfs:subPropertyOf L1:transliteratedOtherEntityName ;
                                         rdfs:domain L1:LegalEntity ;
                                         rdfs:range [ rdf:type rdfs:Datatype ;
                                                      owl:unionOf ( rdf:PlainLiteral
                                                                    xsd:string
                                                                  )
                                                    ] ;
                                         L1:level1CDFFName "PREFERRED_ASCII_TRANSLITERATED_LEGAL_NAME"^^xsd:string ;
                                         L1:level1CDFFType "lei:Tokenized500Type"^^xsd:string ,
                                                           "lei:TransliteratedEntityNameTypeEnum"^^xsd:string ;
                                         rdfs:comment """An element of this type has minimum length of one character and may not contain any of: the carriage return (#xD), line feed (#xA) nor tab (#x9) characters, shall not begin or end with a space (#x20) character, or a sequence of two or more adjacent space characters.

restriction of xs:string
minLength 1
maxLength 500
pattern \\\\S+( \\\\S+)*"""@en ;
                                         rdfs:label "has preferred ASCII-transliterated representation of legal name"@en ;
                                         <http://www.w3.org/2004/02/skos/core#definition> "Legal name of the entity transliterated to ASCII  characters, provided by the entity for this purpose."@en .


###  http://lei.info/voc/l1/previousLegalName
L1:previousLegalName rdf:type owl:DatatypeProperty ;
                     rdfs:subPropertyOf L1:otherEntityName ;
                     rdfs:domain L1:LegalEntity ;
                     rdfs:range [ rdf:type rdfs:Datatype ;
                                  owl:unionOf ( rdf:PlainLiteral
                                                xsd:string
                                              )
                                ] ;
                     L1:level1CDFFName "PREVIOUS_LEGAL_NAME"@en ;
                     L1:level1CDFFType "lei:EntityNameTypeEnum"^^xsd:string ,
                                       "lei:Tokenized500Type"^^xsd:string ;
                     rdfs:comment """An element of this type has minimum length of one character and may not contain any of: the carriage return (#xD), line feed (#xA) nor tab (#x9) characters, shall not begin or end with a space (#x20) character, or a sequence of two or more adjacent space characters.

restriction of xs:string
minLength 1
maxLength 500
pattern \\\\S+( \\\\S+)*"""@en ;
                     rdfs:label "has previous legal name"@en ;
                     <http://www.w3.org/2004/02/skos/core#definition> "A primary legal name previously used by the legal entity."@en .


###  http://lei.info/voc/l1/region
L1:region rdf:type owl:DatatypeProperty ;
          rdfs:subPropertyOf L1:addressDescriptionComponent ;
          rdf:type owl:FunctionalProperty ;
          rdfs:domain L1:Address ;
          rdfs:range xsd:string ;
          L1:level1CDFFName "Region"^^xsd:string ;
          L1:level1CDFFType "lei:RegionCodeType"^^xsd:string ;
          rdfs:comment """minLength 4
maxLength 6
pattern ([A-Z]{2}-[A-Z0-9]{1,3})"""@en ;
          rdfs:label "has subdivision code"@en ;
          <http://www.w3.org/2004/02/skos/core#definition> "The property assigns the 4- to 6-character ISO 3166-2 region code of the region."@en .


###  http://lei.info/voc/l1/registrationAuthorityDescriptionComponent
L1:registrationAuthorityDescriptionComponent rdf:type owl:DatatypeProperty ;
                                             rdfs:label "registration authority description component"@en ;
                                             <http://www.w3.org/2004/02/skos/core#definition> "registration authority description component"@en .


###  http://lei.info/voc/l1/registrationAuthorityEntityID
L1:registrationAuthorityEntityID rdf:type owl:DatatypeProperty ;
                                 rdfs:subPropertyOf L1:registrationAuthorityDescriptionComponent ;
                                 L1:level1CDFFName "RegistrationAuthorityEntityID"^^xsd:string ;
                                 L1:level1CDFFType "lei:Tokenized500Type"^^xsd:string ;
                                 rdfs:comment """An element of this type has minimum length of one character and may not contain any of: the carriage return (#xD), line feed (#xA) nor tab (#x9) characters, shall not begin or end with a space (#x20) character, or a sequence of two or more adjacent space characters.

restriction of xs:string
minLength 1
maxLength 500
pattern \\\\S+( \\\\S+)*"""@en ;
                                 rdfs:label "has validation authority entity ID"@en ;
                                 <http://www.w3.org/2004/02/skos/core#definition> "The identifier of the entity at the indicated registration authority. Typically, the identifier of the legal entity as maintained by a business registry in the jurisdiction of legal registration, or if the entity is one that is not recorded in a business registry (e.g. one of the varieties of funds registered instead with financial regulators), the identifier of the entity in the appropriate registration authority."@en .


###  http://lei.info/voc/l1/registrationAuthorityID
L1:registrationAuthorityID rdf:type owl:DatatypeProperty ;
                           rdfs:subPropertyOf L1:registrationAuthorityDescriptionComponent ;
                           L1:level1CDFFName "RegistrationAuthorityID"^^xsd:string ;
                           L1:level1CDFFType "lei:RegistrationAuthorityEnum"^^xsd:string ;
                           rdfs:comment "pattern RA\\\\d{6}"@en ;
                           rdfs:label "has registration authority ID"@en ;
                           <http://www.w3.org/2004/02/skos/core#definition> "The reference code of the registration authority, taken from the Registration Authorities Code List maintained by GLEIF."@en .


###  http://lei.info/voc/l1/streetAddress
L1:streetAddress rdf:type owl:DatatypeProperty ;
                 rdfs:subPropertyOf L1:addressDescriptionComponent ;
                 rdf:type owl:FunctionalProperty ;
                 rdfs:domain L1:Address ;
                 rdfs:range [ rdf:type rdfs:Datatype ;
                              owl:unionOf ( rdf:PlainLiteral
                                            xsd:string
                                          )
                            ] ;
                 L1:level1CDFFName "AdditionalAddressLine"@en ,
                                   "FirstAddressLine"^^xsd:string ;
                 L1:level1CDFFType "lei:Tokenized500Type"^^xsd:string ;
                 rdfs:comment """An element of this type has minimum length of one character and may not contain any of: the carriage return (#xD), line feed (#xA) nor tab (#x9) characters, shall not begin or end with a space (#x20) character, or a sequence of two or more adjacent space characters.

restriction of xs:string
minLength 1
maxLength 500
pattern \\\\S+( \\\\S+)*"""@en ,
                              "Replaced Line1 by FirstAddressLine and Line2 etc. by AdditionalAddressLine in LEI-CDF 2.0."@en ;
                 rdfs:label "has street address"@en ;
                 <http://www.w3.org/2004/02/skos/core#definition> "The property assigns to the address of legal entity the complete description of the street address."@en .


###  http://lei.info/voc/l1/successorEntityWithoutLEI
L1:successorEntityWithoutLEI rdf:type owl:DatatypeProperty ;
                             rdfs:subPropertyOf L1:legalEntityDescriptionComponent ;
                             rdf:type owl:FunctionalProperty ;
                             rdfs:domain L1:LegalEntity ;
                             rdfs:range [ rdf:type rdfs:Datatype ;
                                          owl:unionOf ( rdf:PlainLiteral
                                                        xsd:string
                                                      )
                                        ] ;
                             L1:level1CDFFName "SuccessorEntity"^^xsd:string ,
                                               "SuccessorEntityName"^^xsd:string ;
                             L1:level1CDFFType "lei:NameType"^^xsd:string ,
                                               "lei:SuccessorEntityType"^^xsd:string ,
                                               "lei:Tokenized500Type"^^xsd:string ;
                             rdfs:comment """An element of this type has minimum length of one character and may not contain any of: the carriage return (#xD), line feed (#xA) nor tab (#x9) characters, shall not begin or end with a space (#x20) character, or a sequence of two or more adjacent space characters.

restriction of xs:string
minLength 1
maxLength 500
pattern \\\\S+( \\\\S+)*"""@en ;
                             rdfs:label "has successor entity with LEI"@en ;
                             <http://www.w3.org/2004/02/skos/core#definition> """The surviving/new legal entity which continues/replaces this registration. 

The successor entity does not have LEI. So the name of the successor entity is assigned."""@en .


###  http://lei.info/voc/l1/tradingOrOperatingName
L1:tradingOrOperatingName rdf:type owl:DatatypeProperty ;
                          rdfs:subPropertyOf L1:otherEntityName ;
                          rdfs:domain L1:LegalEntity ;
                          rdfs:range [ rdf:type rdfs:Datatype ;
                                       owl:unionOf ( rdf:PlainLiteral
                                                     xsd:string
                                                   )
                                     ] ;
                          L1:level1CDFFName "TRADING_OR_OPERATING_NAME"@en ;
                          L1:level1CDFFType "lei:EntityNameTypeEnum"^^xsd:string ,
                                            "lei:Tokenized500Type"^^xsd:string ;
                          rdfs:comment """An element of this type has minimum length of one character and may not contain any of: the carriage return (#xD), line feed (#xA) nor tab (#x9) characters, shall not begin or end with a space (#x20) character, or a sequence of two or more adjacent space characters.

restriction of xs:string
minLength 1
maxLength 500
pattern \\\\S+( \\\\S+)*"""@en ;
                          rdfs:label "has trading or operating name"@en ;
                          <http://www.w3.org/2004/02/skos/core#definition> "A \"trading as\", \"brand name\" or \"operating under\" name currently used by this entity in addition to, but not replacing, the (primary) legal, official registered name."@en .


###  http://lei.info/voc/l1/transliteratedOtherEntityName
L1:transliteratedOtherEntityName rdf:type owl:DatatypeProperty ;
                                 rdfs:subPropertyOf L1:legalEntityDescriptionComponent ,
                                                    L1:name ;
                                 rdfs:domain L1:LegalEntity ;
                                 rdfs:range [ rdf:type rdfs:Datatype ;
                                              owl:unionOf ( rdf:PlainLiteral
                                                            xsd:string
                                                          )
                                            ] ;
                                 L1:level1CDFFName "TransliteratedOtherEntityName"^^xsd:string ,
                                                   "TransliteratedOtherEntityNames"^^xsd:string ;
                                 L1:level1CDFFType "lei:TransliteratedOtherEntityNameType"^^xsd:string ,
                                                   "lei:TransliteratedOtherEntityNamesType"^^xsd:string ;
                                 rdfs:label "has other entity name"@en ;
                                 <http://www.w3.org/2004/02/skos/core#definition> "ASCII-transliterated (i.e. Latin- or Romanized) representation of a name for the legal entity. It is an optional."@en .


###  http://lei.info/voc/l1/validationAuthorityDescriptionComponent
L1:validationAuthorityDescriptionComponent rdf:type owl:DatatypeProperty ;
                                           rdfs:label "validation authority description component"@en ;
                                           <http://www.w3.org/2004/02/skos/core#definition> "validation authority description component"@en .


###  http://lei.info/voc/l1/validationAuthorityEntityID
L1:validationAuthorityEntityID rdf:type owl:DatatypeProperty ;
                               rdfs:subPropertyOf L1:validationAuthorityDescriptionComponent ;
                               rdf:type owl:FunctionalProperty ;
                               rdfs:domain L1:ValidationAuthority ;
                               rdfs:range xsd:string ;
                               L1:level1CDFFName "ValidationAuthorityEntityID"^^xsd:string ;
                               L1:level1CDFFType "lei:Tokenized500Type"^^xsd:string ;
                               rdfs:comment """An element of this type has minimum length of one character and may not contain any of: the carriage return (#xD), line feed (#xA) nor tab (#x9) characters, shall not begin or end with a space (#x20) character, or a sequence of two or more adjacent space characters.

restriction of xs:string
minLength 1
maxLength 500
pattern \\\\S+( \\\\S+)*"""@en ;
                               rdfs:label "has validation authority entity ID"@en ;
                               <http://www.w3.org/2004/02/skos/core#definition> "The identifier of the entity at the indicated registration authority. Typically, the identifier of the legal entity as maintained by a business registry in the jurisdiction of legal registration, or if the entity is one that is not recorded in a business registry (e.g. one of the varieties of funds registered instead with financial regulators), the identifier of the entity in the appropriate registration authority."@en .


###  http://lei.info/voc/l1/validationAuthorityID
L1:validationAuthorityID rdf:type owl:DatatypeProperty ;
                         rdfs:subPropertyOf L1:validationAuthorityDescriptionComponent ;
                         rdf:type owl:FunctionalProperty ;
                         rdfs:domain L1:ValidationAuthority ;
                         rdfs:range xsd:string ;
                         L1:level1CDFFName "ValidationAuthorityID"^^xsd:string ;
                         L1:level1CDFFType "lei:RegistrationAuthorityEnum"^^xsd:string ;
                         rdfs:comment "pattern RA\\\\d{6}"@en ;
                         rdfs:label "has validation authority ID"@en ;
                         <http://www.w3.org/2004/02/skos/core#definition> "The reference code of the registration authority, taken from the Registration Authorities Code List (RAL) maintained by GLEIF."@en .


###  http://lei.info/voc/l2/hasEndDate
L2:hasEndDate rdf:type owl:DatatypeProperty ,
                       owl:FunctionalProperty ;
              rdfs:domain L2:RelationshipPeriodType ;
              rdfs:range xsd:dateTimeStamp ;
              L2:level2CDFFName "EndDate"^^xsd:string ;
              L2:level2CDFFType "LEIDateTimeProfile"^^xsd:string ;
              rdfs:comment """pattern
([^\\\\.]*|([^\\\\.]*(\\\\.((\\\\d){1,3})){0,1}))(Z|\\\\+([01][0- 9]|2[0-3]):([0-5][0-9])|-([01][0-9]|2[0-3]):([0- 5][0-9]))"""@en ;
              rdfs:label "has end date"@en ;
              <http://www.w3.org/2004/02/skos/core#definition> "The end date for a particular period relevant to the relationship."@en .


###  http://lei.info/voc/l2/hasLastUpdateDate
L2:hasLastUpdateDate rdf:type owl:DatatypeProperty ;
                     rdfs:domain L2:Relationship ;
                     rdfs:range xsd:dateTimeStamp ;
                     L2:level2CDFFName "LastUpdateDate"^^xsd:string ;
                     L2:level2CDFFType "rr:LEIDateTimeProfile"^^xsd:string ;
                     rdfs:comment """pattern
([^\\\\.]*|([^\\\\.]*(\\\\.((\\\\d){1,3})){0,1}))(Z|\\\\+([01][0- 9]|2[0-3]):([0-5][0-9])|-([01][0-9]|2[0-3]):([0- 5][0-9]))"""@en ;
                     rdfs:label "has last update date"@en ;
                     <http://www.w3.org/2004/02/skos/core#definition> "The date at which the information was most recently updated by the managing LOU."@en .


###  http://lei.info/voc/l2/initialRegistrationDate
L2:initialRegistrationDate rdf:type owl:DatatypeProperty ;
                           rdfs:domain L2:Relationship ;
                           rdfs:range xsd:dateTimeStamp ;
                           L2:level2CDFFName "InitialRegistrationDate"^^xsd:string ;
                           L2:level2CDFFType "rr:LEIDateTimeProfile"^^xsd:string ;
                           rdfs:comment """pattern
([^\\\\.]*|([^\\\\.]*(\\\\.((\\\\d){1,3})){0,1}))(Z|\\\\+([01][0- 9]|2[0-3]):([0-5][0-9])|-([01][0-9]|2[0-3]):([0- 5][0-9]))"""@en ;
                           rdfs:label "has initial registration date"@en ;
                           <http://www.w3.org/2004/02/skos/core#definition> "The date at which the relationship information was first collected by the managing LOU."@en .


###  http://lei.info/voc/l2/nextRenewalDate
L2:nextRenewalDate rdf:type owl:DatatypeProperty ;
                   rdfs:domain L2:Relationship ;
                   rdfs:range xsd:dateTimeStamp ;
                   L2:level2CDFFName "NextRenewalDate"^^xsd:string ;
                   L2:level2CDFFType "rr:LEIDateTimeProfile"^^xsd:string ;
                   rdfs:comment """pattern
([^\\\\.]*|([^\\\\.]*(\\\\.((\\\\d){1,3})){0,1}))(Z|\\\\+([01][0- 9]|2[0-3]):([0-5][0-9])|-([01][0-9]|2[0-3]):([0- 5][0-9]))"""@en ;
                   rdfs:label "has next renewal date"@en ;
                   <http://www.w3.org/2004/02/skos/core#definition> "The next date by which the relationship information must be renewed and re-certified by the legal entity."@en .


###  http://lei.info/voc/l2/quantifierAmount
L2:quantifierAmount rdf:type owl:DatatypeProperty ,
                             owl:FunctionalProperty ;
                    rdfs:domain L2:RelationshipQuantifier ;
                    rdfs:range xsd:decimal ;
                    L2:level2CDFFName "QuantifierAmount"^^xsd:string ;
                    L2:level2CDFFType "xs:decimal"^^xsd:string ;
                    rdfs:label "has quantifier amount"@en ;
                    <http://www.w3.org/2004/02/skos/core#definition> "This property specifies the quantity measured as a decimal (positive or negative) number, using a \".\" as the decimal point, with no spaces, and without thousand delimiters (e.g. \",\")."@en .


###  http://lei.info/voc/l2/startDate
L2:startDate rdf:type owl:DatatypeProperty ,
                      owl:FunctionalProperty ;
             rdfs:domain L2:RelationshipPeriodType ;
             rdfs:range xsd:dateTimeStamp ;
             L2:level2CDFFName "StartDate"^^xsd:string ;
             L2:level2CDFFType "LEIDateTimeProfile"^^xsd:string ;
             rdfs:comment """pattern
([^\\\\.]*|([^\\\\.]*(\\\\.((\\\\d){1,3})){0,1}))(Z|\\\\+([01][0- 9]|2[0-3]):([0-5][0-9])|-([01][0-9]|2[0-3]):([0- 5][0-9]))"""@en ;
             rdfs:label "has start date"@en ;
             <http://www.w3.org/2004/02/skos/core#definition> "The start date for a particular period relevant to the relationship."@en .


###  http://lei.info/voc/l2/validationReference
L2:validationReference rdf:type owl:DatatypeProperty ;
                       rdfs:domain L2:Relationship ;
                       rdfs:range xsd:anyURI ;
                       L2:level2CDFFName "ValidationReference"^^xsd:string ;
                       L2:level2CDFFType "rr:Tokenized500Type"^^xsd:string ;
                       rdfs:comment """An element of this type has minimum length of one character and may not contain any of: the carriage return (#xD), line feed (#xA) nor tab (#x9) characters, shall not begin or end with a space (#x20) character, or a sequence of two or more adjacent space characters.

restriction of xs:string
minLength 1
maxLength 500
pattern \\\\S+( \\\\S+)*"""@en ;
                       rdfs:label "has validation reference"@en ;
                       <http://www.w3.org/2004/02/skos/core#definition> "This property specifies a reference to a specific document or other source used as the basis of relationship validation for this relationship record."@en .


#################################################################
#    Classes
#################################################################

###  http://lei.info/voc/l1/Address
L1:Address rdf:type owl:Class ;
           rdfs:subClassOf [ owl:intersectionOf ( [ rdf:type owl:Restriction ;
                                                    owl:onProperty L1:addressNumber ;
                                                    owl:minQualifiedCardinality "0"^^xsd:nonNegativeInteger ;
                                                    owl:onDataRange [ rdf:type rdfs:Datatype ;
                                                                      owl:unionOf ( rdf:PlainLiteral
                                                                                    xsd:string
                                                                                  )
                                                                    ]
                                                  ]
                                                  [ rdf:type owl:Restriction ;
                                                    owl:onProperty L1:addressNumber ;
                                                    owl:maxQualifiedCardinality "1"^^xsd:nonNegativeInteger ;
                                                    owl:onDataRange [ rdf:type rdfs:Datatype ;
                                                                      owl:unionOf ( rdf:PlainLiteral
                                                                                    xsd:string
                                                                                  )
                                                                    ]
                                                  ]
                                                ) ;
                             rdf:type owl:Class
                           ] ,
                           [ owl:intersectionOf ( [ rdf:type owl:Restriction ;
                                                    owl:onProperty L1:addressNumberWithinBuilding ;
                                                    owl:minQualifiedCardinality "0"^^xsd:nonNegativeInteger ;
                                                    owl:onDataRange [ rdf:type rdfs:Datatype ;
                                                                      owl:unionOf ( rdf:PlainLiteral
                                                                                    xsd:string
                                                                                  )
                                                                    ]
                                                  ]
                                                  [ rdf:type owl:Restriction ;
                                                    owl:onProperty L1:addressNumberWithinBuilding ;
                                                    owl:maxQualifiedCardinality "1"^^xsd:nonNegativeInteger ;
                                                    owl:onDataRange [ rdf:type rdfs:Datatype ;
                                                                      owl:unionOf ( rdf:PlainLiteral
                                                                                    xsd:string
                                                                                  )
                                                                    ]
                                                  ]
                                                ) ;
                             rdf:type owl:Class
                           ] ,
                           [ owl:intersectionOf ( [ rdf:type owl:Restriction ;
                                                    owl:onProperty L1:mailRouting ;
                                                    owl:minQualifiedCardinality "0"^^xsd:nonNegativeInteger ;
                                                    owl:onDataRange [ rdf:type rdfs:Datatype ;
                                                                      owl:unionOf ( rdf:PlainLiteral
                                                                                    xsd:string
                                                                                  )
                                                                    ]
                                                  ]
                                                  [ rdf:type owl:Restriction ;
                                                    owl:onProperty L1:mailRouting ;
                                                    owl:maxQualifiedCardinality "1"^^xsd:nonNegativeInteger ;
                                                    owl:onDataRange [ rdf:type rdfs:Datatype ;
                                                                      owl:unionOf ( rdf:PlainLiteral
                                                                                    xsd:string
                                                                                  )
                                                                    ]
                                                  ]
                                                ) ;
                             rdf:type owl:Class
                           ] ,
                           [ owl:intersectionOf ( [ rdf:type owl:Restriction ;
                                                    owl:onProperty L1:postalCode ;
                                                    owl:minQualifiedCardinality "0"^^xsd:nonNegativeInteger ;
                                                    owl:onDataRange [ rdf:type rdfs:Datatype ;
                                                                      owl:unionOf ( rdf:PlainLiteral
                                                                                    xsd:string
                                                                                  )
                                                                    ]
                                                  ]
                                                  [ rdf:type owl:Restriction ;
                                                    owl:onProperty L1:postalCode ;
                                                    owl:maxQualifiedCardinality "1"^^xsd:nonNegativeInteger ;
                                                    owl:onDataRange [ rdf:type rdfs:Datatype ;
                                                                      owl:unionOf ( rdf:PlainLiteral
                                                                                    xsd:string
                                                                                  )
                                                                    ]
                                                  ]
                                                ) ;
                             rdf:type owl:Class
                           ] ,
                           [ owl:intersectionOf ( [ rdf:type owl:Restriction ;
                                                    owl:onProperty L1:region ;
                                                    owl:minQualifiedCardinality "0"^^xsd:nonNegativeInteger ;
                                                    owl:onDataRange xsd:string
                                                  ]
                                                  [ rdf:type owl:Restriction ;
                                                    owl:onProperty L1:region ;
                                                    owl:maxQualifiedCardinality "1"^^xsd:nonNegativeInteger ;
                                                    owl:onDataRange xsd:string
                                                  ]
                                                ) ;
                             rdf:type owl:Class
                           ] ,
                           [ rdf:type owl:Restriction ;
                             owl:onProperty L1:city ;
                             owl:qualifiedCardinality "1"^^xsd:nonNegativeInteger ;
                             owl:onDataRange [ rdf:type rdfs:Datatype ;
                                               owl:unionOf ( rdf:PlainLiteral
                                                             xsd:string
                                                           )
                                             ]
                           ] ,
                           [ rdf:type owl:Restriction ;
                             owl:onProperty L1:country ;
                             owl:qualifiedCardinality "1"^^xsd:nonNegativeInteger ;
                             owl:onDataRange xsd:string
                           ] ,
                           [ rdf:type owl:Restriction ;
                             owl:onProperty L1:streetAddress ;
                             owl:qualifiedCardinality "1"^^xsd:nonNegativeInteger ;
                             owl:onDataRange [ rdf:type rdfs:Datatype ;
                                               owl:unionOf ( rdf:PlainLiteral
                                                             xsd:string
                                                           )
                                             ]
                           ] ;
           L1:level1CDFFName "HeadquartersAddress"^^xsd:string ,
                             "LegalAddress"^^xsd:string ,
                             "OtherAddresses"^^xsd:string ,
                             "TransliteratedOtherAddresses"^^xsd:string ;
           L1:level1CDFFType "lei:AddressType"^^xsd:string ;
           rdfs:label "address"@en ;
           <http://www.w3.org/2004/02/skos/core#definition> "An address is a geographical location of Legal Entity. It is specified by providing information about country, subdivision, city, street or postal code. Legal Entity can have many addresses: the address of legal formation, the address of the headquarters of the entity and others. The role of the address of the legal entity is specified by object properties such as :hasLegalAddress and :hasHeadquartersAddress."@en ;
           <http://www.w3.org/2004/02/skos/core#exactMatch> "http://schema.org/Address"^^xsd:anyURI .


###  http://lei.info/voc/l1/EntityCategory
L1:EntityCategory rdf:type owl:Class ;
                  L1:level1CDFFName "EntityCategory"^^xsd:string ;
                  L1:level1CDFFType "lei:EntityCategoryTypeEnum"^^xsd:string ;
                  rdfs:label "legal entity category"@en ;
                  <http://www.w3.org/2004/02/skos/core#definition> """Indicates the category of entity. 

These categories are based on use cases specified in LEI-ROC policies, found at http://www.leiroc.org/list/leiroc_gls/index.htm"""@en .


###  http://lei.info/voc/l1/EntityExpirationReason
L1:EntityExpirationReason rdf:type owl:Class ;
                          L1:level1CDFFName "EntityExpirationReason"^^xsd:string ;
                          L1:level1CDFFType "lei:EntityExpirationReasonEnum"^^xsd:string ;
                          rdfs:comment "Entity expiration reason shall be assigned to a legal entity if the legal entity expired and omitted otherwise. If a legal entity expired, then the entity expiration reason shall be assigned to the legal entity together with its expiration date (see :hasEntityExpirationDate data property)."@en ;
                          rdfs:label "entity expiration reason"@en ;
                          <http://www.w3.org/2004/02/skos/core#definition> "A legal entity expiration reason is a reason that a legal entity ceased to exist and/or operate."@en .


###  http://lei.info/voc/l1/EntityStatus
L1:EntityStatus rdf:type owl:Class ;
                L1:level1CDFFName "EntityStatus"^^xsd:string ;
                L1:level1CDFFType "lei:EntityStatusEnum"^^xsd:string ;
                rdfs:label "entity status"@en ;
                <http://www.w3.org/2004/02/skos/core#definition> "A legal entity status is a status of the legal entity. There are two possible values of the status: \"active\" or \"inactive\". This is not to be confused with the status of the general legal entity identifier registration (see :RegistrationStatus). If a legal entity is related by :successorLegalEntity with other legal entity, then its legal entity status is the last status of the legal entity before this record was superseded. This status is not necessarily the current status of the legal entity."@en .


###  http://lei.info/voc/l1/LegalEntity
L1:LegalEntity rdf:type owl:Class ;
               owl:equivalentClass L2:LegalEntity ;
               rdfs:subClassOf [ owl:intersectionOf ( [ rdf:type owl:Restriction ;
                                                        owl:onProperty L1:entityCategory ;
                                                        owl:minQualifiedCardinality "0"^^xsd:nonNegativeInteger ;
                                                        owl:onClass L1:EntityCategory
                                                      ]
                                                      [ rdf:type owl:Restriction ;
                                                        owl:onProperty L1:entityCategory ;
                                                        owl:maxQualifiedCardinality "1"^^xsd:nonNegativeInteger ;
                                                        owl:onClass L1:EntityCategory
                                                      ]
                                                    ) ;
                                 rdf:type owl:Class
                               ] ,
                               [ owl:intersectionOf ( [ rdf:type owl:Restriction ;
                                                        owl:onProperty L1:entityExpirationReason ;
                                                        owl:minQualifiedCardinality "0"^^xsd:nonNegativeInteger ;
                                                        owl:onClass L1:EntityExpirationReason
                                                      ]
                                                      [ rdf:type owl:Restriction ;
                                                        owl:onProperty L1:entityExpirationReason ;
                                                        owl:maxQualifiedCardinality "1"^^xsd:nonNegativeInteger ;
                                                        owl:onClass L1:EntityExpirationReason
                                                      ]
                                                    ) ;
                                 rdf:type owl:Class
                               ] ,
                               [ owl:intersectionOf ( [ rdf:type owl:Restriction ;
                                                        owl:onProperty L1:fundFamily ;
                                                        owl:minQualifiedCardinality "0"^^xsd:nonNegativeInteger ;
                                                        owl:onClass L1:LegalEntity
                                                      ]
                                                      [ rdf:type owl:Restriction ;
                                                        owl:onProperty L1:fundFamily ;
                                                        owl:maxQualifiedCardinality "1"^^xsd:nonNegativeInteger ;
                                                        owl:onClass L1:LegalEntity
                                                      ]
                                                    ) ;
                                 rdf:type owl:Class
                               ] ,
                               [ owl:intersectionOf ( [ rdf:type owl:Restriction ;
                                                        owl:onProperty L1:identifiedBy ;
                                                        owl:minQualifiedCardinality "0"^^xsd:nonNegativeInteger ;
                                                        owl:onClass L1:LegalEntityIdentifier
                                                      ]
                                                      [ rdf:type owl:Restriction ;
                                                        owl:onProperty L1:identifiedBy ;
                                                        owl:maxQualifiedCardinality "1"^^xsd:nonNegativeInteger ;
                                                        owl:onClass L1:LegalEntityIdentifier
                                                      ]
                                                    ) ;
                                 rdf:type owl:Class
                               ] ,
                               [ owl:intersectionOf ( [ rdf:type owl:Restriction ;
                                                        owl:onProperty L1:primaryValidationAuthority ;
                                                        owl:minQualifiedCardinality "0"^^xsd:nonNegativeInteger ;
                                                        owl:onClass L1:ValidationAuthority
                                                      ]
                                                      [ rdf:type owl:Restriction ;
                                                        owl:onProperty L1:primaryValidationAuthority ;
                                                        owl:maxQualifiedCardinality "1"^^xsd:nonNegativeInteger ;
                                                        owl:onClass L1:ValidationAuthority
                                                      ]
                                                    ) ;
                                 rdf:type owl:Class
                               ] ,
                               [ owl:intersectionOf ( [ rdf:type owl:Restriction ;
                                                        owl:onProperty L1:registrationAuthority ;
                                                        owl:minQualifiedCardinality "0"^^xsd:nonNegativeInteger ;
                                                        owl:onClass L1:RegistrationAuthority
                                                      ]
                                                      [ rdf:type owl:Restriction ;
                                                        owl:onProperty L1:registrationAuthority ;
                                                        owl:maxQualifiedCardinality "1"^^xsd:nonNegativeInteger ;
                                                        owl:onClass L1:RegistrationAuthority
                                                      ]
                                                    ) ;
                                 rdf:type owl:Class
                               ] ,
                               [ owl:intersectionOf ( [ rdf:type owl:Restriction ;
                                                        owl:onProperty L1:successorEntityWithLEI ;
                                                        owl:minQualifiedCardinality "0"^^xsd:nonNegativeInteger ;
                                                        owl:onClass L1:LegalEntity
                                                      ]
                                                      [ rdf:type owl:Restriction ;
                                                        owl:onProperty L1:successorEntityWithLEI ;
                                                        owl:maxQualifiedCardinality "1"^^xsd:nonNegativeInteger ;
                                                        owl:onClass L1:LegalEntity
                                                      ]
                                                    ) ;
                                 rdf:type owl:Class
                               ] ,
                               [ owl:intersectionOf ( [ rdf:type owl:Restriction ;
                                                        owl:onProperty L1:validationSource ;
                                                        owl:minQualifiedCardinality "0"^^xsd:nonNegativeInteger ;
                                                        owl:onClass L1:ValidationSource
                                                      ]
                                                      [ rdf:type owl:Restriction ;
                                                        owl:onProperty L1:validationSource ;
                                                        owl:maxQualifiedCardinality "1"^^xsd:nonNegativeInteger ;
                                                        owl:onClass L1:ValidationSource
                                                      ]
                                                    ) ;
                                 rdf:type owl:Class
                               ] ,
                               [ owl:intersectionOf ( [ rdf:type owl:Restriction ;
                                                        owl:onProperty L1:entityExpirationDate ;
                                                        owl:minQualifiedCardinality "0"^^xsd:nonNegativeInteger ;
                                                        owl:onDataRange xsd:dateTime
                                                      ]
                                                      [ rdf:type owl:Restriction ;
                                                        owl:onProperty L1:entityExpirationDate ;
                                                        owl:maxQualifiedCardinality "1"^^xsd:nonNegativeInteger ;
                                                        owl:onDataRange xsd:dateTimeStamp
                                                      ]
                                                    ) ;
                                 rdf:type owl:Class
                               ] ,
                               [ owl:intersectionOf ( [ rdf:type owl:Restriction ;
                                                        owl:onProperty L1:entityLegalFormCode ;
                                                        owl:minQualifiedCardinality "0"^^xsd:nonNegativeInteger ;
                                                        owl:onDataRange xsd:string
                                                      ]
                                                      [ rdf:type owl:Restriction ;
                                                        owl:onProperty L1:entityLegalFormCode ;
                                                        owl:maxQualifiedCardinality "1"^^xsd:nonNegativeInteger ;
                                                        owl:onDataRange xsd:string
                                                      ]
                                                    ) ;
                                 rdf:type owl:Class
                               ] ,
                               [ owl:intersectionOf ( [ rdf:type owl:Restriction ;
                                                        owl:onProperty L1:fundFamilyWithoutLEI ;
                                                        owl:minQualifiedCardinality "0"^^xsd:nonNegativeInteger ;
                                                        owl:onDataRange [ rdf:type rdfs:Datatype ;
                                                                          owl:unionOf ( rdf:PlainLiteral
                                                                                        xsd:string
                                                                                      )
                                                                        ]
                                                      ]
                                                      [ rdf:type owl:Restriction ;
                                                        owl:onProperty L1:fundFamilyWithoutLEI ;
                                                        owl:maxQualifiedCardinality "1"^^xsd:nonNegativeInteger ;
                                                        owl:onDataRange [ rdf:type rdfs:Datatype ;
                                                                          owl:unionOf ( rdf:PlainLiteral
                                                                                        xsd:string
                                                                                      )
                                                                        ]
                                                      ]
                                                    ) ;
                                 rdf:type owl:Class
                               ] ,
                               [ owl:intersectionOf ( [ rdf:type owl:Restriction ;
                                                        owl:onProperty L1:legalJurisdiction ;
                                                        owl:minQualifiedCardinality "0"^^xsd:nonNegativeInteger ;
                                                        owl:onDataRange xsd:string
                                                      ]
                                                      [ rdf:type owl:Restriction ;
                                                        owl:onProperty L1:legalJurisdiction ;
                                                        owl:maxQualifiedCardinality "1"^^xsd:nonNegativeInteger ;
                                                        owl:onDataRange xsd:string
                                                      ]
                                                    ) ;
                                 rdf:type owl:Class
                               ] ,
                               [ owl:intersectionOf ( [ rdf:type owl:Restriction ;
                                                        owl:onProperty L1:otherLegalForm ;
                                                        owl:minQualifiedCardinality "0"^^xsd:nonNegativeInteger ;
                                                        owl:onDataRange xsd:string
                                                      ]
                                                      [ rdf:type owl:Restriction ;
                                                        owl:onProperty L1:otherLegalForm ;
                                                        owl:maxQualifiedCardinality "1"^^xsd:nonNegativeInteger ;
                                                        owl:onDataRange xsd:string
                                                      ]
                                                    ) ;
                                 rdf:type owl:Class
                               ] ,
                               [ owl:intersectionOf ( [ rdf:type owl:Restriction ;
                                                        owl:onProperty L1:successorEntityWithoutLEI ;
                                                        owl:minQualifiedCardinality "0"^^xsd:nonNegativeInteger ;
                                                        owl:onDataRange [ rdf:type rdfs:Datatype ;
                                                                          owl:unionOf ( rdf:PlainLiteral
                                                                                        xsd:string
                                                                                      )
                                                                        ]
                                                      ]
                                                      [ rdf:type owl:Restriction ;
                                                        owl:onProperty L1:successorEntityWithoutLEI ;
                                                        owl:maxQualifiedCardinality "1"^^xsd:nonNegativeInteger ;
                                                        owl:onDataRange [ rdf:type rdfs:Datatype ;
                                                                          owl:unionOf ( rdf:PlainLiteral
                                                                                        xsd:string
                                                                                      )
                                                                        ]
                                                      ]
                                                    ) ;
                                 rdf:type owl:Class
                               ] ,
                               [ rdf:type owl:Restriction ;
                                 owl:onProperty L1:alternativeLanguageHeadquartersAddress ;
                                 owl:minQualifiedCardinality "0"^^xsd:nonNegativeInteger ;
                                 owl:onClass L1:Address
                               ] ,
                               [ rdf:type owl:Restriction ;
                                 owl:onProperty L1:alternativeLanguageLegalAddress ;
                                 owl:minQualifiedCardinality "0"^^xsd:nonNegativeInteger ;
                                 owl:onClass L1:Address
                               ] ,
                               [ rdf:type owl:Restriction ;
                                 owl:onProperty L1:autoASCIITransliteratedHeadquartersAddress ;
                                 owl:minQualifiedCardinality "0"^^xsd:nonNegativeInteger ;
                                 owl:onClass L1:Address
                               ] ,
                               [ rdf:type owl:Restriction ;
                                 owl:onProperty L1:autoASCIITransliteratedLegalAddress ;
                                 owl:minQualifiedCardinality "0"^^xsd:nonNegativeInteger ;
                                 owl:onClass L1:Address
                               ] ,
                               [ rdf:type owl:Restriction ;
                                 owl:onProperty L1:otherValidationAuthority ;
                                 owl:minQualifiedCardinality "0"^^xsd:nonNegativeInteger ;
                                 owl:onClass L1:ValidationAuthority
                               ] ,
                               [ rdf:type owl:Restriction ;
                                 owl:onProperty L1:preferredASCIITransliteratedHeadquartersAddress ;
                                 owl:minQualifiedCardinality "0"^^xsd:nonNegativeInteger ;
                                 owl:onClass L1:Address
                               ] ,
                               [ rdf:type owl:Restriction ;
                                 owl:onProperty L1:preferredASCIITransliteratedLegalAddress ;
                                 owl:minQualifiedCardinality "0"^^xsd:nonNegativeInteger ;
                                 owl:onClass L1:Address
                               ] ,
                               [ rdf:type owl:Restriction ;
                                 owl:onProperty L1:headquartersAddress ;
                                 owl:qualifiedCardinality "1"^^xsd:nonNegativeInteger ;
                                 owl:onClass L1:Address
                               ] ,
                               [ rdf:type owl:Restriction ;
                                 owl:onProperty L1:legalAddress ;
                                 owl:qualifiedCardinality "1"^^xsd:nonNegativeInteger ;
                                 owl:onClass L1:Address
                               ] ,
                               [ rdf:type owl:Restriction ;
                                 owl:onProperty L1:legalEntityStatus ;
                                 owl:qualifiedCardinality "1"^^xsd:nonNegativeInteger ;
                                 owl:onClass L1:EntityStatus
                               ] ,
                               [ rdf:type owl:Restriction ;
                                 owl:onProperty L1:alternativeLanguageEntityName ;
                                 owl:minQualifiedCardinality "0"^^xsd:nonNegativeInteger ;
                                 owl:onDataRange [ rdf:type rdfs:Datatype ;
                                                   owl:unionOf ( rdf:PlainLiteral
                                                                 xsd:string
                                                               )
                                                 ]
                               ] ,
                               [ rdf:type owl:Restriction ;
                                 owl:onProperty L1:autoASCIITransliteratedLegalName ;
                                 owl:minQualifiedCardinality "0"^^xsd:nonNegativeInteger ;
                                 owl:onDataRange [ rdf:type rdfs:Datatype ;
                                                   owl:unionOf ( rdf:PlainLiteral
                                                                 xsd:string
                                                               )
                                                 ]
                               ] ,
                               [ rdf:type owl:Restriction ;
                                 owl:onProperty L1:preferredASCIITransliteratedLegalName ;
                                 owl:minQualifiedCardinality "0"^^xsd:nonNegativeInteger ;
                                 owl:onDataRange [ rdf:type rdfs:Datatype ;
                                                   owl:unionOf ( rdf:PlainLiteral
                                                                 xsd:string
                                                               )
                                                 ]
                               ] ,
                               [ rdf:type owl:Restriction ;
                                 owl:onProperty L1:previousLegalName ;
                                 owl:minQualifiedCardinality "0"^^xsd:nonNegativeInteger ;
                                 owl:onDataRange [ rdf:type rdfs:Datatype ;
                                                   owl:unionOf ( rdf:PlainLiteral
                                                                 xsd:string
                                                               )
                                                 ]
                               ] ,
                               [ rdf:type owl:Restriction ;
                                 owl:onProperty L1:tradingOrOperatingName ;
                                 owl:minQualifiedCardinality "0"^^xsd:nonNegativeInteger ;
                                 owl:onDataRange [ rdf:type rdfs:Datatype ;
                                                   owl:unionOf ( rdf:PlainLiteral
                                                                 xsd:string
                                                               )
                                                 ]
                               ] ,
                               [ rdf:type owl:Restriction ;
                                 owl:onProperty L1:legalName ;
                                 owl:qualifiedCardinality "1"^^xsd:nonNegativeInteger ;
                                 owl:onDataRange [ rdf:type rdfs:Datatype ;
                                                   owl:unionOf ( rdf:PlainLiteral
                                                                 xsd:string
                                                               )
                                                 ]
                               ] ;
               L1:level1CDFFName "Entity"^^xsd:string ;
               L1:level1CDFFType "lei:EntityType"^^xsd:string ;
               rdfs:label "legal entity"@en ;
               <http://www.w3.org/2004/02/skos/core#definition> """Legal entity is a partnership, corporation, or other organization having the capacity to negotiate contracts, assume financial obligations, and pay off debts, organized under the laws of some jurisdiction. (FIBO)

Legal entity is characterised in GLEIS by its reference data, enabling its identification."""@en ,
                                                                "The Entity container element contains the legal entity's reference data, enabling identification."@en ;
               <http://www.w3.org/2004/02/skos/core#exactMatch> "http://schema.org/Organization"^^xsd:anyURI .


###  http://lei.info/voc/l1/LegalEntityIdentifier
L1:LegalEntityIdentifier rdf:type owl:Class ;
                         rdfs:subClassOf [ rdf:type owl:Restriction ;
                                           owl:onProperty L1:identifies ;
                                           owl:qualifiedCardinality "1"^^xsd:nonNegativeInteger ;
                                           owl:onClass L1:LegalEntity
                                         ] ,
                                         [ rdf:type owl:Restriction ;
                                           owl:onProperty L1:managingLOU ;
                                           owl:qualifiedCardinality "1"^^xsd:nonNegativeInteger ;
                                           owl:onClass L1:LocalOperatingUnit
                                         ] ,
                                         [ rdf:type owl:Restriction ;
                                           owl:onProperty L1:registrationStatus ;
                                           owl:qualifiedCardinality "1"^^xsd:nonNegativeInteger ;
                                           owl:onClass L1:RegistrationStatus
                                         ] ,
                                         [ rdf:type owl:Restriction ;
                                           owl:onProperty L1:initialRegistrationDate ;
                                           owl:qualifiedCardinality "1"^^xsd:nonNegativeInteger ;
                                           owl:onDataRange xsd:dateTimeStamp
                                         ] ,
                                         [ rdf:type owl:Restriction ;
                                           owl:onProperty L1:lastUpdateDate ;
                                           owl:qualifiedCardinality "1"^^xsd:nonNegativeInteger ;
                                           owl:onDataRange xsd:dateTimeStamp
                                         ] ,
                                         [ rdf:type owl:Restriction ;
                                           owl:onProperty L1:leiCode ;
                                           owl:qualifiedCardinality "1"^^xsd:nonNegativeInteger ;
                                           owl:onDataRange xsd:string
                                         ] ,
                                         [ rdf:type owl:Restriction ;
                                           owl:onProperty L1:nextRenewalDate ;
                                           owl:qualifiedCardinality "1"^^xsd:nonNegativeInteger ;
                                           owl:onDataRange xsd:dateTimeStamp
                                         ] ;
                         L1:level1CDFFName "LEI"^^xsd:string ;
                         L1:level1CDFFType "lei:LEIType"@en ;
                         rdfs:comment "Any registration of identifier of legal entity"@en ;
                         rdfs:label "legal entity identifier"@en ;
                         <http://www.w3.org/2004/02/skos/core#definition> "A global legal entity identifier (GLEI) specifies identifier of the legal entity as maintained by a local operating unit (LOU). A complete registration of GLEI provides a unique 20-character alphanumeric code based on the ISO 17442 standard and attributes describing the registration of this GLEI with the LOU."@en .


###  http://lei.info/voc/l1/LocalOperatingUnit
L1:LocalOperatingUnit rdf:type owl:Class ;
                      owl:equivalentClass L2:LocalOperatingUnit ;
                      rdfs:subClassOf L1:LegalEntity ,
                                      [ rdf:type owl:Restriction ;
                                        owl:onProperty [ owl:inverseOf L1:managingLOU
                                                       ] ;
                                        owl:someValuesFrom L1:LegalEntityIdentifier
                                      ] ;
                      L1:level1CDFFName "ManagingLOU"^^xsd:string ;
                      L1:level1CDFFType "lei:LEIType"^^xsd:string ;
                      rdfs:label "local operating unit"@en ;
                      <http://www.w3.org/2004/02/skos/core#definition> "The LOU is a registration authority that is responsible for administering  registration of LEIs."@en .


###  http://lei.info/voc/l1/RegistrationAuthority
L1:RegistrationAuthority rdf:type owl:Class ;
                         rdfs:subClassOf [ owl:intersectionOf ( [ rdf:type owl:Restriction ;
                                                                  owl:onProperty L1:otherRegistrationAuthorityID ;
                                                                  owl:minQualifiedCardinality "0"^^xsd:nonNegativeInteger ;
                                                                  owl:onDataRange xsd:string
                                                                ]
                                                                [ rdf:type owl:Restriction ;
                                                                  owl:onProperty L1:otherRegistrationAuthorityID ;
                                                                  owl:maxQualifiedCardinality "1"^^xsd:nonNegativeInteger ;
                                                                  owl:onDataRange xsd:string
                                                                ]
                                                              ) ;
                                           rdf:type owl:Class
                                         ] ,
                                         [ owl:intersectionOf ( [ rdf:type owl:Restriction ;
                                                                  owl:onProperty L1:registrationAuthorityEntityID ;
                                                                  owl:minQualifiedCardinality "0"^^xsd:nonNegativeInteger ;
                                                                  owl:onDataRange xsd:string
                                                                ]
                                                                [ rdf:type owl:Restriction ;
                                                                  owl:onProperty L1:registrationAuthorityEntityID ;
                                                                  owl:maxQualifiedCardinality "1"^^xsd:nonNegativeInteger ;
                                                                  owl:onDataRange xsd:string
                                                                ]
                                                              ) ;
                                           rdf:type owl:Class
                                         ] ,
                                         [ rdf:type owl:Restriction ;
                                           owl:onProperty L1:registrationAuthorityID ;
                                           owl:qualifiedCardinality "1"^^xsd:nonNegativeInteger ;
                                           owl:onDataRange xsd:string
                                         ] ;
                         L1:level1CDFFName "RegistrationAuthority"^^xsd:string ;
                         L1:level1CDFFType "lei:RegistrationAuthorityType"^^xsd:string ;
                         rdfs:label "registration authority"@en ;
                         <http://www.w3.org/2004/02/skos/core#definition> "An identifier for the legal entity in a business registry in the jurisdiction of legal registration, or in the appropriate registration authority."@en .


###  http://lei.info/voc/l1/RegistrationStatus
L1:RegistrationStatus rdf:type owl:Class ;
                      L1:level1CDFFName "RegistrationStatus"^^xsd:string ;
                      L1:level1CDFFType "lei:RegistrationStatusEnum"^^xsd:string ;
                      rdfs:label "registration status"@en ;
                      <http://www.w3.org/2004/02/skos/core#definition> "The status of the legal entity's LEI registration with the Managing LOU."@en .


###  http://lei.info/voc/l1/ValidationAuthority
L1:ValidationAuthority rdf:type owl:Class ;
                       rdfs:subClassOf [ owl:intersectionOf ( [ rdf:type owl:Restriction ;
                                                                owl:onProperty L1:otherValidationAuthorityID ;
                                                                owl:minQualifiedCardinality "0"^^xsd:nonNegativeInteger ;
                                                                owl:onDataRange xsd:string
                                                              ]
                                                              [ rdf:type owl:Restriction ;
                                                                owl:onProperty L1:otherValidationAuthorityID ;
                                                                owl:maxQualifiedCardinality "1"^^xsd:nonNegativeInteger ;
                                                                owl:onDataRange xsd:string
                                                              ]
                                                            ) ;
                                         rdf:type owl:Class
                                       ] ,
                                       [ owl:intersectionOf ( [ rdf:type owl:Restriction ;
                                                                owl:onProperty L1:validationAuthorityEntityID ;
                                                                owl:minQualifiedCardinality "0"^^xsd:nonNegativeInteger ;
                                                                owl:onDataRange xsd:string
                                                              ]
                                                              [ rdf:type owl:Restriction ;
                                                                owl:onProperty L1:validationAuthorityEntityID ;
                                                                owl:maxQualifiedCardinality "1"^^xsd:nonNegativeInteger ;
                                                                owl:onDataRange xsd:string
                                                              ]
                                                            ) ;
                                         rdf:type owl:Class
                                       ] ,
                                       [ rdf:type owl:Restriction ;
                                         owl:onProperty L1:validationAuthorityID ;
                                         owl:qualifiedCardinality "1"^^xsd:nonNegativeInteger ;
                                         owl:onDataRange xsd:string
                                       ] ;
                       L1:level1CDFFName "ValidationAuthority"^^xsd:string ;
                       L1:level1CDFFType "lei:ValidationAuthorityType"^^xsd:string ;
                       rdfs:label "validation authority"@en ;
                       <http://www.w3.org/2004/02/skos/core#definition> "The (primary) registration authority used by the LOU to validate the entity data."@en .


###  http://lei.info/voc/l1/ValidationSource
L1:ValidationSource rdf:type owl:Class ;
                    L1:level1CDFFName "ValidationSources"^^xsd:string ;
                    L1:level1CDFFType "lei:ValidationSourcesEnum"^^xsd:string ;
                    rdfs:label "validation source"@en ;
                    <http://www.w3.org/2004/02/skos/core#definition> "The level of validation of the reference data provided by the registrant."@en .


###  http://lei.info/voc/l2/AccountingPeriod
L2:AccountingPeriod rdf:type owl:Class ;
                    rdfs:subClassOf L2:RelationshipPeriodType ,
                                    [ owl:intersectionOf ( [ rdf:type owl:Restriction ;
                                                             owl:onProperty L2:hasEndDate ;
                                                             owl:minQualifiedCardinality "0"^^xsd:nonNegativeInteger ;
                                                             owl:onDataRange xsd:dateTime
                                                           ]
                                                           [ rdf:type owl:Restriction ;
                                                             owl:onProperty L2:hasEndDate ;
                                                             owl:maxQualifiedCardinality "1"^^xsd:nonNegativeInteger ;
                                                             owl:onDataRange xsd:dateTime
                                                           ]
                                                         ) ;
                                      rdf:type owl:Class
                                    ] ,
                                    [ owl:intersectionOf ( [ rdf:type owl:Restriction ;
                                                             owl:onProperty L2:startDate ;
                                                             owl:minQualifiedCardinality "0"^^xsd:nonNegativeInteger ;
                                                             owl:onDataRange xsd:dateTime
                                                           ]
                                                           [ rdf:type owl:Restriction ;
                                                             owl:onProperty L2:startDate ;
                                                             owl:maxQualifiedCardinality "1"^^xsd:nonNegativeInteger ;
                                                             owl:onDataRange xsd:dateTime
                                                           ]
                                                         ) ;
                                      rdf:type owl:Class
                                    ] ;
                    L2:level2CDFFName "ACCOUNTING_PERIOD"^^xsd:string ,
                                      "RelationshipPeriod"^^xsd:string ;
                    L2:level2CDFFType "PeriodTypeEnum"^^xsd:string ,
                                      "rr:RelationshipPeriodType"^^xsd:string ;
                    rdfs:label "accounting period"@en ;
                    <http://www.w3.org/2004/02/skos/core#definition> "The dates in this instance of RelationshipPeriod indicate the accounting period covered by the most recent validation documents for this relationship."@en .


###  http://lei.info/voc/l2/DocumentFilingPeriod
L2:DocumentFilingPeriod rdf:type owl:Class ;
                        rdfs:subClassOf L2:RelationshipPeriodType ,
                                        [ owl:intersectionOf ( [ rdf:type owl:Restriction ;
                                                                 owl:onProperty L2:hasEndDate ;
                                                                 owl:minQualifiedCardinality "0"^^xsd:nonNegativeInteger ;
                                                                 owl:onDataRange xsd:dateTime
                                                               ]
                                                               [ rdf:type owl:Restriction ;
                                                                 owl:onProperty L2:hasEndDate ;
                                                                 owl:maxQualifiedCardinality "1"^^xsd:nonNegativeInteger ;
                                                                 owl:onDataRange xsd:dateTime
                                                               ]
                                                             ) ;
                                          rdf:type owl:Class
                                        ] ,
                                        [ owl:intersectionOf ( [ rdf:type owl:Restriction ;
                                                                 owl:onProperty L2:startDate ;
                                                                 owl:minQualifiedCardinality "0"^^xsd:nonNegativeInteger ;
                                                                 owl:onDataRange xsd:dateTime
                                                               ]
                                                               [ rdf:type owl:Restriction ;
                                                                 owl:onProperty L2:startDate ;
                                                                 owl:maxQualifiedCardinality "1"^^xsd:nonNegativeInteger ;
                                                                 owl:onDataRange xsd:dateTime
                                                               ]
                                                             ) ;
                                          rdf:type owl:Class
                                        ] ;
                        L2:level2CDFFName "DOCUMENT_FILING_PERIOD"^^xsd:string ,
                                          "RelationshipPeriod"^^xsd:string ;
                        L2:level2CDFFType "PeriodTypeEnum"^^xsd:string ,
                                          "rr:RelationshipPeriodType"^^xsd:string ;
                        rdfs:label "document filing period"@en ;
                        <http://www.w3.org/2004/02/skos/core#definition> "The dates in this instance of RelationshipPeriod indicate the validity period of a regulatory filing, accounting document, or other document demonstrating the relationship's validity."@en .


###  http://lei.info/voc/l2/LegalEntity
L2:LegalEntity rdf:type owl:Class ;
               L2:level2CDFFName "NodeID"^^xsd:string ;
               L2:level2CDFFType "rr:LEIType"^^xsd:string ;
               rdfs:label "managing LOU"@en ;
               <http://www.w3.org/2004/02/skos/core#definition> "The legal entity participating in the relationship."@en ;
               <http://www.w3.org/2004/02/skos/core#exactMatch> "http://schema.org/Organization"^^xsd:anyURI .


###  http://lei.info/voc/l2/LocalOperatingUnit
L2:LocalOperatingUnit rdf:type owl:Class ;
                      rdfs:subClassOf L2:LegalEntity ;
                      L2:level2CDFFName "ManagingLOU"^^xsd:string ;
                      L2:level2CDFFType "rr:LEIType"^^xsd:string ;
                      rdfs:label "local operating unit"@en ;
                      <http://www.w3.org/2004/02/skos/core#definition> "The LOU that is responsible for administering this relationship record."@en .


###  http://lei.info/voc/l2/MeasurementMethod
L2:MeasurementMethod rdf:type owl:Class ;
                     L2:level2CDFFName "MeasurementMethod"^^xsd:string ;
                     L2:level2CDFFType "rr:RelationshipQuantifierType"^^xsd:string ;
                     rdfs:label "measurement method"@en ;
                     <http://www.w3.org/2004/02/skos/core#definition> "Specifies the method of measurement (or set of rules) used to quantitatively categorize the relationship."@en .


###  http://lei.info/voc/l2/RegistrationStatus
L2:RegistrationStatus rdf:type owl:Class ;
                      L2:level2CDFFName "RegistrationStatus"^^xsd:string ;
                      L2:level2CDFFType "rr:RegistrationStatusEnum"^^xsd:string ;
                      rdfs:label "relationship registration status"@en ;
                      <http://www.w3.org/2004/02/skos/core#definition> "The status of the legal entity's relationship record registration with the managing LOU."@en .


###  http://lei.info/voc/l2/Relationship
L2:Relationship rdf:type owl:Class ;
                rdfs:subClassOf [ owl:intersectionOf ( [ rdf:type owl:Restriction ;
                                                         owl:onProperty L2:relationshipPeriod ;
                                                         owl:minQualifiedCardinality "0"^^xsd:nonNegativeInteger ;
                                                         owl:onClass L2:RelationshipPeriodType
                                                       ]
                                                       [ rdf:type owl:Restriction ;
                                                         owl:onProperty L2:relationshipPeriod ;
                                                         owl:maxQualifiedCardinality "1"^^xsd:nonNegativeInteger ;
                                                         owl:onClass L2:RelationshipPeriodType
                                                       ]
                                                     ) ;
                                  rdf:type owl:Class
                                ] ,
                                [ owl:intersectionOf ( [ rdf:type owl:Restriction ;
                                                         owl:onProperty L2:nextRenewalDate ;
                                                         owl:minQualifiedCardinality "0"^^xsd:nonNegativeInteger ;
                                                         owl:onDataRange xsd:dateTimeStamp
                                                       ]
                                                       [ rdf:type owl:Restriction ;
                                                         owl:onProperty L2:nextRenewalDate ;
                                                         owl:maxQualifiedCardinality "1"^^xsd:nonNegativeInteger ;
                                                         owl:onDataRange xsd:dateTimeStamp
                                                       ]
                                                     ) ;
                                  rdf:type owl:Class
                                ] ,
                                [ owl:intersectionOf ( [ rdf:type owl:Restriction ;
                                                         owl:onProperty L2:validationReference ;
                                                         owl:minQualifiedCardinality "0"^^xsd:nonNegativeInteger ;
                                                         owl:onDataRange xsd:anyURI
                                                       ]
                                                       [ rdf:type owl:Restriction ;
                                                         owl:onProperty L2:validationReference ;
                                                         owl:maxQualifiedCardinality "1"^^xsd:nonNegativeInteger ;
                                                         owl:onDataRange xsd:anyURI
                                                       ]
                                                     ) ;
                                  rdf:type owl:Class
                                ] ,
                                [ rdf:type owl:Restriction ;
                                  owl:onProperty L2:relationshipQualifier ;
                                  owl:minQualifiedCardinality "0"^^xsd:nonNegativeInteger ;
                                  owl:onClass L2:RelationshipQualifier
                                ] ,
                                [ rdf:type owl:Restriction ;
                                  owl:onProperty L2:relationshipQuantifier ;
                                  owl:minQualifiedCardinality "0"^^xsd:nonNegativeInteger ;
                                  owl:onClass L2:RelationshipQuantifier
                                ] ,
                                [ rdf:type owl:Restriction ;
                                  owl:onProperty L2:childLegalEntity ;
                                  owl:qualifiedCardinality "1"^^xsd:nonNegativeInteger ;
                                  owl:onClass L2:LegalEntity
                                ] ,
                                [ rdf:type owl:Restriction ;
                                  owl:onProperty L2:managingLOU ;
                                  owl:qualifiedCardinality "1"^^xsd:nonNegativeInteger ;
                                  owl:onClass L2:LocalOperatingUnit
                                ] ,
                                [ rdf:type owl:Restriction ;
                                  owl:onProperty L2:parentLegalEntity ;
                                  owl:qualifiedCardinality "1"^^xsd:nonNegativeInteger ;
                                  owl:onClass L2:LegalEntity
                                ] ,
                                [ rdf:type owl:Restriction ;
                                  owl:onProperty L2:registrationStatus ;
                                  owl:qualifiedCardinality "1"^^xsd:nonNegativeInteger ;
                                  owl:onClass L2:RegistrationStatus
                                ] ,
                                [ rdf:type owl:Restriction ;
                                  owl:onProperty L2:relationshipStatus ;
                                  owl:qualifiedCardinality "1"^^xsd:nonNegativeInteger ;
                                  owl:onClass L2:RelationshipStatus
                                ] ,
                                [ rdf:type owl:Restriction ;
                                  owl:onProperty L2:relationshipType ;
                                  owl:qualifiedCardinality "1"^^xsd:nonNegativeInteger ;
                                  owl:onClass L2:RelationshipType
                                ] ,
                                [ rdf:type owl:Restriction ;
                                  owl:onProperty L2:validationDocument ;
                                  owl:qualifiedCardinality "1"^^xsd:nonNegativeInteger ;
                                  owl:onClass L2:ValidationDocument
                                ] ,
                                [ rdf:type owl:Restriction ;
                                  owl:onProperty L2:hasLastUpdateDate ;
                                  owl:qualifiedCardinality "1"^^xsd:nonNegativeInteger ;
                                  owl:onDataRange xsd:dateTimeStamp
                                ] ,
                                [ rdf:type owl:Restriction ;
                                  owl:onProperty L2:initialRegistrationDate ;
                                  owl:qualifiedCardinality "1"^^xsd:nonNegativeInteger ;
                                  owl:onDataRange xsd:dateTimeStamp
                                ] ;
                L2:level2CDFFName "Relationship"^^xsd:string ;
                L2:level2CDFFType "rr:RelationshipContainerType"^^xsd:string ;
                rdfs:label "relationship"@en ;
                rdfs:seeAlso <http://lei.info/gleio/rr/RelationshipManifestation> ;
                <http://www.w3.org/2004/02/skos/core#definition> "It identifiers two entities related by the reported relationship, as well as the type of relationship, dates related to the relationship and other relationship quantifiers and qualifiers."@en .


###  http://lei.info/voc/l2/RelationshipPeriod
L2:RelationshipPeriod rdf:type owl:Class ;
                      rdfs:subClassOf L2:RelationshipPeriodType ,
                                      [ owl:intersectionOf ( [ rdf:type owl:Restriction ;
                                                               owl:onProperty L2:hasEndDate ;
                                                               owl:minQualifiedCardinality "0"^^xsd:nonNegativeInteger ;
                                                               owl:onDataRange xsd:dateTime
                                                             ]
                                                             [ rdf:type owl:Restriction ;
                                                               owl:onProperty L2:hasEndDate ;
                                                               owl:maxQualifiedCardinality "1"^^xsd:nonNegativeInteger ;
                                                               owl:onDataRange xsd:dateTime
                                                             ]
                                                           ) ;
                                        rdf:type owl:Class
                                      ] ,
                                      [ owl:intersectionOf ( [ rdf:type owl:Restriction ;
                                                               owl:onProperty L2:startDate ;
                                                               owl:minQualifiedCardinality "0"^^xsd:nonNegativeInteger ;
                                                               owl:onDataRange xsd:dateTime
                                                             ]
                                                             [ rdf:type owl:Restriction ;
                                                               owl:onProperty L2:startDate ;
                                                               owl:maxQualifiedCardinality "1"^^xsd:nonNegativeInteger ;
                                                               owl:onDataRange xsd:dateTime
                                                             ]
                                                           ) ;
                                        rdf:type owl:Class
                                      ] ;
                      L2:level2CDFFName "RELATIONSHIP_PERIOD"^^xsd:string ,
                                        "RelationshipPeriod"^^xsd:string ;
                      L2:level2CDFFType "PeriodTypeEnum"^^xsd:string ,
                                        "rr:RelationshipPeriodType"^^xsd:string ;
                      rdfs:label "relationship period"@en ;
                      <http://www.w3.org/2004/02/skos/core#definition> "The dates in this instance of RelationshipPeriod indicate the duration of validity of the relationship itself, as distinct from any administrative or reporting aspects."@en .


###  http://lei.info/voc/l2/RelationshipPeriodType
L2:RelationshipPeriodType rdf:type owl:Class ;
                          rdfs:subClassOf [ owl:intersectionOf ( [ rdf:type owl:Restriction ;
                                                                   owl:onProperty L2:hasEndDate ;
                                                                   owl:minQualifiedCardinality "0"^^xsd:nonNegativeInteger ;
                                                                   owl:onDataRange xsd:dateTime
                                                                 ]
                                                                 [ rdf:type owl:Restriction ;
                                                                   owl:onProperty L2:hasEndDate ;
                                                                   owl:maxQualifiedCardinality "1"^^xsd:nonNegativeInteger ;
                                                                   owl:onDataRange xsd:dateTime
                                                                 ]
                                                               ) ;
                                            rdf:type owl:Class
                                          ] ,
                                          [ owl:intersectionOf ( [ rdf:type owl:Restriction ;
                                                                   owl:onProperty L2:startDate ;
                                                                   owl:minQualifiedCardinality "0"^^xsd:nonNegativeInteger ;
                                                                   owl:onDataRange xsd:dateTime
                                                                 ]
                                                                 [ rdf:type owl:Restriction ;
                                                                   owl:onProperty L2:startDate ;
                                                                   owl:maxQualifiedCardinality "1"^^xsd:nonNegativeInteger ;
                                                                   owl:onDataRange xsd:dateTime
                                                                 ]
                                                               ) ;
                                            rdf:type owl:Class
                                          ] ;
                          L2:level2CDFFName "RelationshipPeriod"^^xsd:string ;
                          L2:level2CDFFType "rr:RelationshipPeriodType"^^xsd:string ;
                          rdfs:label "relationship period"@en ;
                          <http://www.w3.org/2004/02/skos/core#definition> "Contains start and end dates for a particular type of period, for example, the duration of the relationship itself, the filing or validity period of any documents demonstrating the relationship, or the accounting period they refer to."@en .


###  http://lei.info/voc/l2/RelationshipQualifier
L2:RelationshipQualifier rdf:type owl:Class ;
                         rdfs:subClassOf [ owl:intersectionOf ( [ rdf:type owl:Restriction ;
                                                                  owl:onProperty L2:qualifierCategory ;
                                                                  owl:minQualifiedCardinality "0"^^xsd:nonNegativeInteger ;
                                                                  owl:onClass L2:RelationshipQualifierCategory
                                                                ]
                                                                [ rdf:type owl:Restriction ;
                                                                  owl:onProperty L2:qualifierCategory ;
                                                                  owl:maxQualifiedCardinality "1"^^xsd:nonNegativeInteger ;
                                                                  owl:onClass L2:RelationshipQualifierCategory
                                                                ]
                                                              ) ;
                                           rdf:type owl:Class
                                         ] ,
                                         [ rdf:type owl:Restriction ;
                                           owl:onProperty L2:qualifierDimension ;
                                           owl:qualifiedCardinality "1"^^xsd:nonNegativeInteger ;
                                           owl:onClass L2:RelationshipQualifierDimension
                                         ] ;
                         L2:level2CDFFName "RelationshipQualifier"^^xsd:string ;
                         L2:level2CDFFType "rr:RelationshipQualifiersType"^^xsd:string ;
                         rdfs:label "relationship qualifier"@en ;
                         <http://www.w3.org/2004/02/skos/core#definition> "Any additional qualitative attributes that help to categorize the relationship."@en .


###  http://lei.info/voc/l2/RelationshipQualifierCategory
L2:RelationshipQualifierCategory rdf:type owl:Class ;
                                 L2:level2CDFFName "QualifierCategory"^^xsd:string ;
                                 L2:level2CDFFType "rr:QualifierCategoryTypeEnum"^^xsd:string ;
                                 rdfs:label "qualifier category"@en ;
                                 <http://www.w3.org/2004/02/skos/core#definition> "Specifies the additional qualitative attributes that help to categorize the relationship."@en .


###  http://lei.info/voc/l2/RelationshipQualifierDimension
L2:RelationshipQualifierDimension rdf:type owl:Class ;
                                  L2:level2CDFFName "QualifierDimension"^^xsd:string ;
                                  L2:level2CDFFType "rr:QualifierDimensionEnum"^^xsd:string ;
                                  rdfs:label "qualifier dimension"@en ;
                                  <http://www.w3.org/2004/02/skos/core#definition> "Designates the optional list of additional qualitative attributes that help to categorize the relationship."@en .


###  http://lei.info/voc/l2/RelationshipQuantifier
L2:RelationshipQuantifier rdf:type owl:Class ;
                          rdfs:subClassOf [ owl:intersectionOf ( [ rdf:type owl:Restriction ;
                                                                   owl:onProperty L2:quantifierUnit ;
                                                                   owl:minQualifiedCardinality "0"^^xsd:nonNegativeInteger ;
                                                                   owl:onClass L2:RelationshipQuantifierUnit
                                                                 ]
                                                                 [ rdf:type owl:Restriction ;
                                                                   owl:onProperty L2:quantifierUnit ;
                                                                   owl:maxQualifiedCardinality "1"^^xsd:nonNegativeInteger ;
                                                                   owl:onClass L2:RelationshipQuantifierUnit
                                                                 ]
                                                               ) ;
                                            rdf:type owl:Class
                                          ] ,
                                          [ rdf:type owl:Restriction ;
                                            owl:onProperty L2:measurementMethod ;
                                            owl:qualifiedCardinality "1"^^xsd:nonNegativeInteger ;
                                            owl:onClass L2:MeasurementMethod
                                          ] ,
                                          [ rdf:type owl:Restriction ;
                                            owl:onProperty L2:quantifierAmount ;
                                            owl:qualifiedCardinality "1"^^xsd:nonNegativeInteger ;
                                            owl:onDataRange xsd:decimal
                                          ] ;
                          L2:level2CDFFName "RelationshipQuantifier"^^xsd:string ;
                          L2:level2CDFFType "rr:RelationshipQuantifierType"^^xsd:string ;
                          rdfs:label "relationship quantifier"@en ;
                          <http://www.w3.org/2004/02/skos/core#definition> "Any additional quantitative attributes that help to categorize the relationship."@en .


###  http://lei.info/voc/l2/RelationshipQuantifierUnit
L2:RelationshipQuantifierUnit rdf:type owl:Class ;
                              L2:level2CDFFName "QuantifierUnits"^^xsd:string ;
                              L2:level2CDFFType "QuantifierUnitsTypeEnum"^^xsd:string ;
                              rdfs:label "quantifier unit"@en ;
                              <http://www.w3.org/2004/02/skos/core#definition> "Specifies the units, where applicable, of a measurement made on a relationship."@en .


###  http://lei.info/voc/l2/RelationshipStatus
L2:RelationshipStatus rdf:type owl:Class ;
                      L2:level2CDFFName "RelationshipStatus"^^xsd:string ;
                      L2:level2CDFFType "rr:RelationshipStatusEnum"^^xsd:string ;
                      rdfs:label "relationship status"@en ;
                      <http://www.w3.org/2004/02/skos/core#definition> "The status of the legal entities' relationship itself: ACTIVE or INACTIVE."@en .


###  http://lei.info/voc/l2/RelationshipType
L2:RelationshipType rdf:type owl:Class ;
                    L2:level2CDFFName "RelationshipType"^^xsd:string ;
                    L2:level2CDFFType "rr:RelationshipTypeEnum"^^xsd:string ;
                    rdfs:label "relationship type"@en ;
                    <http://www.w3.org/2004/02/skos/core#definition> "A unique code designating the specific category of a directional relationship between two legal entities."@en .


###  http://lei.info/voc/l2/ValidationDocument
L2:ValidationDocument rdf:type owl:Class ;
                      L2:level2CDFFName "ValidationDocuments"^^xsd:string ;
                      L2:level2CDFFType "rr:ValidationDocumentsTypeEnum"^^xsd:string ;
                      rdfs:label "relationship validation document type"@en ;
                      <http://www.w3.org/2004/02/skos/core#definition> "Type of source document(s) used for validating the relationship."@en .


###  http://lei.info/voc/l2/ValidationSource
L2:ValidationSource rdf:type owl:Class ;
                    L2:level2CDFFName "ValidationSources"^^xsd:string ;
                    L2:level2CDFFType "rr:ValidationSourcesTypeEnum"^^xsd:string ;
                    rdfs:label "relationship validation source"@en ;
                    <http://www.w3.org/2004/02/skos/core#definition> "Level of relationship validation."@en .


#################################################################
#    Individuals
#################################################################

###  http://lei.info/voc/l1/Active
L1:Active rdf:type owl:NamedIndividual ,
                   L1:EntityStatus ;
          L1:level1CDFFName "ACTIVE"^^xsd:string ;
          L1:level1CDFFType "lei:EntityStatusEnum"^^xsd:string ;
          rdfs:label "Active"@en ;
          <http://www.w3.org/2004/02/skos/core#definition> "As of the last report or update, the legal entity reported that is was legally registered and operating."@en .


###  http://lei.info/voc/l1/Annulled
L1:Annulled rdf:type owl:NamedIndividual ,
                     L1:RegistrationStatus ;
            L1:level1CDFFName "ANNULLED"^^xsd:string ;
            L1:level1CDFFType "lei:RegistrationStatusEnum"^^xsd:string ;
            rdfs:label "Annulled"@en ;
            <http://www.w3.org/2004/02/skos/core#definition> "A global legal entity identifier registration that was marked as erroneous or invalid after it was issued."@en .


###  http://lei.info/voc/l1/Branch
L1:Branch rdf:type owl:NamedIndividual ,
                   L1:EntityCategory ;
          L1:level1CDFFName "BRANCH"^^xsd:string ,
                            "EntityCategoryTypeEnum"^^xsd:string ;
          L1:level1CDFFType "lei:EntityCategoryTypeEnum"^^xsd:string ;
          rdfs:label "branch"@en ;
          <http://www.w3.org/2004/02/skos/core#definition> "The legal entity is a branch of another legal entity."@en .


###  http://lei.info/voc/l1/Cancelled
L1:Cancelled rdf:type owl:NamedIndividual ,
                      L1:RegistrationStatus ;
             L1:level1CDFFName "CANCELLED"^^xsd:string ;
             L1:level1CDFFType "lei:RegistrationStatusEnum"^^xsd:string ;
             rdfs:label "Cancelled"@en ;
             <http://www.w3.org/2004/02/skos/core#definition> "A global legal entity identifier registration that was abandoned prior to issuance of a global legal entity identifier."@en .


###  http://lei.info/voc/l1/CorporateAction
L1:CorporateAction rdf:type owl:NamedIndividual ,
                            L1:EntityExpirationReason ;
                   L1:level1CDFFName "CORPORATE_ACTION"^^xsd:string ;
                   L1:level1CDFFType "lei:EntityExpirationReasonEnum"^^xsd:string ;
                   rdfs:label "Corporate Action"@en ;
                   <http://www.w3.org/2004/02/skos/core#definition> "The legal entity was acquired or merged with another legal entity."@en .


###  http://lei.info/voc/l1/Dissolved
L1:Dissolved rdf:type owl:NamedIndividual ,
                      L1:EntityExpirationReason ;
             L1:level1CDFFName "DISSOLVED"^^xsd:string ;
             L1:level1CDFFType "lei:EntityExpirationReasonEnum"^^xsd:string ;
             rdfs:label "Dissolved"@en ;
             <http://www.w3.org/2004/02/skos/core#definition> "The legal entity ceased to operate."@en .


###  http://lei.info/voc/l1/Duplicate
L1:Duplicate rdf:type owl:NamedIndividual ,
                      L1:RegistrationStatus ;
             L1:level1CDFFName "DUPLICATE"^^xsd:string ;
             L1:level1CDFFType "lei:RegistrationStatusEnum"^^xsd:string ;
             rdfs:comment """The DUPLICATE status is assigned to the non-surviving registration (i.e., the LEI that should no longer be used). 

Only one of the potential multiple identifiers will survive; for all other duplicate registrations:
1. The RegistrationStatus is set to DUPLICATE
2. The LEI of the surviving LEI Registration is set in the SuccessorLEI data element of (each) duplicate LEI registration
3. The LastUpdateDate is set to reflect the date of this update
4. No further updates of the DUPLICATE registration record will occur"""@en ;
             rdfs:label "Duplicate"@en ;
             <http://www.w3.org/2004/02/skos/core#definition> "A global legal entity identifier registration that has been determined to be a duplicate registration of the same legal entity as another global legal entity identifier registration."@en .


###  http://lei.info/voc/l1/EntitySuppliedOnly
L1:EntitySuppliedOnly rdf:type owl:NamedIndividual ,
                               L1:ValidationSource ;
                      L1:level1CDFFName "ENTITY_SUPPLIED_ONLY"^^xsd:string ;
                      L1:level1CDFFType "lei:ValidationSourcesEnum"^^xsd:string ;
                      rdfs:label "Entity Supplied Only"@en ;
                      <http://www.w3.org/2004/02/skos/core#definition> "Based on the validation procedures in use by the local operating unit responsible for the record, the information associated with this record has significant reliance on the information that a submitter provided due to the unavailability of corroborating information."@en .


###  http://lei.info/voc/l1/FullyCorroborated
L1:FullyCorroborated rdf:type owl:NamedIndividual ,
                              L1:ValidationSource ;
                     L1:level1CDFFName "FULLY_CORROBORATED"^^xsd:string ;
                     L1:level1CDFFType "lei:ValidationSourcesEnum"^^xsd:string ;
                     rdfs:label "Fully Corroborated"@en ;
                     <http://www.w3.org/2004/02/skos/core#definition> "Based on the validation procedures in use by the local operating unit responsible for the record, there is sufficient information contained in authoritative public sources to corroborate the information that the submitter has provided for the record."@en .


###  http://lei.info/voc/l1/Fund
L1:Fund rdf:type owl:NamedIndividual ,
                 L1:EntityCategory ;
        L1:level1CDFFName "EntityCategoryTypeEnum"^^xsd:string ,
                          "FUND"^^xsd:string ;
        L1:level1CDFFType "lei:EntityCategoryTypeEnum"^^xsd:string ;
        rdfs:label "fund"@en ;
        <http://www.w3.org/2004/02/skos/core#definition> "The legal entity is a fund managed by another legal entity."@en .


###  http://lei.info/voc/l1/Inactive
L1:Inactive rdf:type owl:NamedIndividual ,
                     L1:EntityStatus ;
            L1:level1CDFFName "INACTIVE"^^xsd:string ;
            L1:level1CDFFType "lei:EntityStatusEnum"^^xsd:string ;
            rdfs:label "Inactive"@en ;
            <http://www.w3.org/2004/02/skos/core#definition> """It has been determined that the legal entity that was assigned the global legal entity identifier is no longer legally registered and/or operating, whether as a result of:
1. Business closure
2. Acquisition by or merger with another (or new) entity
3. Determination of illegitimacy."""@en .


###  http://lei.info/voc/l1/Issued
L1:Issued rdf:type owl:NamedIndividual ,
                   L1:RegistrationStatus ;
          L1:level1CDFFName "ISSUED"^^xsd:string ;
          L1:level1CDFFType "lei:RegistrationStatusEnum"^^xsd:string ;
          rdfs:label "Issued"@en ;
          <http://www.w3.org/2004/02/skos/core#definition> "A global legal entity identifier registration that has been validated and issued, and which identifies an entity that was an operating legal entity as of the last update."@en .


###  http://lei.info/voc/l1/Lapsed
L1:Lapsed rdf:type owl:NamedIndividual ,
                   L1:RegistrationStatus ;
          L1:level1CDFFName "LAPSED"^^xsd:string ;
          L1:level1CDFFType "lei:RegistrationStatusEnum"^^xsd:string ;
          rdfs:comment """After being issued an LEI, an entity must regularly do the following:
- Periodically verify the continued accuracy of its registration reference data that is recorded in the LOU that is responsible for managing the LEI registration of the entity, updating any aspect of the registration reference data that has changed;
- Periodically renew its LEI registration agreement with the LOU, paying the renewal fee.

(Although both of the above actions are typically performed at the same time, it is certainly possible that the frequency of each action could be different.) If, after being issued an LEI,

- A legal entity fails to renew and re-certify its LEI registration with the LOU responsible to manage the registration by the leiNextRenewalDate, and
- The legal entity fails to do so for a pre-determined (as yet unspecified) period of time, and
- The legal entity is not known by public sources to have ceased operation

Then
1. The leiRegistrationStatus is set to LAPSED,
2. Updates to the LEI registration are permitted, notably to reinstate the registration to the ISSUED status."""@en ;
          rdfs:label "Lapsed"@en ;
          <http://www.w3.org/2004/02/skos/core#definition> "A global legal entity identifier registration that has not been renewed and has exceeded any allowed grace period for renewal."@en .


###  http://lei.info/voc/l1/Merged
L1:Merged rdf:type owl:NamedIndividual ,
                   L1:RegistrationStatus ;
          L1:level1CDFFName "MERGED"^^xsd:string ;
          L1:level1CDFFType "lei:RegistrationStatusEnum"^^xsd:string ;
          rdfs:comment """If
- After being issued an LEI, the entity is acquired by, or merged with, another legal entity;
- Per agreements among the parties to the transaction, the LEI of the acquired or merged entity will not be used to identify the surviving entity (or if a new entity is created that is issued a new LEI)

Then
1. The leiRegistrationStatus is set to MERGED,
2. The LEI of the surviving/new legal entity is set in the successorLEI data element of (each) LEI registration that is no longer to be used;
3. The leiRecordLastUpdate is set to reflect the date of this update,
4. The EntityExpirationDate is also set to the date of this update,
5. The EntityExpirationReason is set to CORPORATE_ACTION,
6. The EntityStatus is set to INACTIVE; and
7. No further updates of the MERGED registration record(s) will occur."""@en ;
          rdfs:label "Merged"@en ;
          <http://www.w3.org/2004/02/skos/core#definition> "A global legal entity identifier registration for an entity that has been merged into another legal entity, such that this legal entity no longer exists as an operating entity."@en .


###  http://lei.info/voc/l1/Other
L1:Other rdf:type owl:NamedIndividual ,
                  L1:EntityExpirationReason ;
         L1:level1CDFFName "OTHER"^^xsd:string ;
         L1:level1CDFFType "lei:EntityExpirationReasonEnum"^^xsd:string ;
         rdfs:label "Other"@en ;
         <http://www.w3.org/2004/02/skos/core#definition> "The reason for expiry is not corporate action or dissolved."@en .


###  http://lei.info/voc/l1/PartiallyCorroborated
L1:PartiallyCorroborated rdf:type owl:NamedIndividual ,
                                  L1:ValidationSource ;
                         L1:level1CDFFName "PARTIALLY_CORROBORATED"^^xsd:string ;
                         L1:level1CDFFType "lei:ValidationSourcesEnum"^^xsd:string ;
                         rdfs:label "Fully Corroborated"@en ,
                                    "Partially Corroborated"@en ;
                         <http://www.w3.org/2004/02/skos/core#definition> "Based on the validation procedures in use by the local operating unit responsible for the record, the information supplied by the registrant can be partially corroborated by public authoritative sources, while some of the record is dependent upon the information that the registrant submitted, either due to conflicts with authoritative information, or due to data unavailability."@en .


###  http://lei.info/voc/l1/Pending
L1:Pending rdf:type owl:NamedIndividual ,
                    L1:ValidationSource ;
           L1:level1CDFFName "PENDING"^^xsd:string ;
           L1:level1CDFFType "lei:ValidationSourcesEnum"^^xsd:string ;
           rdfs:label "Pending"@en ;
           <http://www.w3.org/2004/02/skos/core#definition> "The validation of the reference data provided by the registrant has not yet occurred."@en .


###  http://lei.info/voc/l1/PendingArchival
L1:PendingArchival rdf:type owl:NamedIndividual ,
                            L1:RegistrationStatus ;
                   L1:level1CDFFName "PENDING_ARCHIVAL"^^xsd:string ;
                   L1:level1CDFFType "lei:RegistrationStatusEnum"^^xsd:string ;
                   rdfs:label "Pending Archival"@en ;
                   <http://www.w3.org/2004/02/skos/core#definition> "A global legal entity identifier registration is about to be transferred to a different local operating unit, after which its registration status will revert to a non-pending status. The pending archival status serves to inform recipients of local operating unit provided data files that a global legal entity identifier record will be removed from that local operating units published file after the transfer is complete."@en .


###  http://lei.info/voc/l1/PendingTransfer
L1:PendingTransfer rdf:type owl:NamedIndividual ,
                            L1:RegistrationStatus ;
                   L1:level1CDFFName "PENDING_TRANSFER"^^xsd:string ;
                   L1:level1CDFFType "lei:RegistrationStatusEnum"^^xsd:string ;
                   rdfs:label "Pending Transfer"@en ;
                   <http://www.w3.org/2004/02/skos/core#definition> "A global legal entity identifier registration that has been requested to be transferred to another local operating unit. The request is being processed at the sending local operating unit. When the receiving local operating unit is ready, the status will be changed to pending archival by the sending local operating unit prior to completion of the transfer."@en .


###  http://lei.info/voc/l1/PendingValidation
L1:PendingValidation rdf:type owl:NamedIndividual ,
                              L1:RegistrationStatus ;
                     L1:level1CDFFName "PENDING_VALIDATION"^^xsd:string ;
                     L1:level1CDFFType "lei:RegistrationStatusEnum"^^xsd:string ;
                     rdfs:isDefinedBy "LEI Data File Format 1.0, section: 3.5.7." ;
                     rdfs:label "Pending Validation"@en ;
                     <http://www.w3.org/2004/02/skos/core#definition> "An application for a global legal entity identifier that has been submitted and which is being processed and validated. A global legal entity identifier registrations in the pending state are not intended for public release, but could be used internally between local operating units."@en .


###  http://lei.info/voc/l1/Retired
L1:Retired rdf:type owl:NamedIndividual ,
                    L1:RegistrationStatus ;
           L1:level1CDFFName "RETIRED"^^xsd:string ;
           L1:level1CDFFType "lei:RegistrationStatusEnum"^^xsd:string ;
           rdfs:comment """If
- After being issued an LEI, the entity ceases to operate (goes out of business and/or dissolves its legal standing)
- The entity informs the LOU of the cessation of business, OR, the managing LOU determines by public sources that the legal entity has been dissolved or ceased to operate (and the LOU seeks to confirm this status through all available channels with the entity)

Then
1. The leiRegistrationStatus is set to RETIRED;
2. The leiRecordLastUpdate is set to reflect the date of this update;
3. The EntityExpirationDate is also set to the date of this update;
4. The EntityExpirationReason is set to DISSOLVED;
5. The EntityStatus is set to INACTIVE; and
6. No further updates of the RETIRED registration record will occur."""@en ;
           rdfs:label "Retired"@en ;
           <http://www.w3.org/2004/02/skos/core#definition> "A global legal entity identifier registration for an entity that has ceased operation, without having been merged into another entity."@en .


###  http://lei.info/voc/l1/SoleProprietor
L1:SoleProprietor rdf:type owl:NamedIndividual ,
                           L1:EntityCategory ;
                  L1:level1CDFFName "EntityCategoryTypeEnum"^^xsd:string ,
                                    "SOLE_PROPRIETOR"^^xsd:string ;
                  L1:level1CDFFType "lei:EntityCategoryTypeEnum"^^xsd:string ;
                  rdfs:label "sole proprietor"@en ;
                  <http://www.w3.org/2004/02/skos/core#definition> "The legal entity is an individual acting in a business capacity."@en .


###  http://lei.info/voc/l1/Transferred
L1:Transferred rdf:type owl:NamedIndividual ,
                        L1:RegistrationStatus ;
               L1:level1CDFFName "TRANSFERRED"^^xsd:string ;
               L1:level1CDFFType "lei:RegistrationStatusEnum"^^xsd:string ;
               rdfs:label "Transferred"@en ;
               <http://www.w3.org/2004/02/skos/core#definition> "A global legal entity identifier registration that has been transferred to a different local operating unit as the managing local operating unit. A record in this state is not published, but may be used internally by the prior local operating unit for audit trail purposes."@en .


###  http://lei.info/voc/l2/AccountingConsolidation
L2:AccountingConsolidation rdf:type owl:NamedIndividual ,
                                    L2:MeasurementMethod ;
                           L2:level2CDFFName "ACCOUNTING_CONSOLIDATION"^^xsd:string ;
                           L2:level2CDFFType "rr:RelationshipQuantifierType"^^xsd:string ;
                           rdfs:label "measurement method"@en ;
                           <http://www.w3.org/2004/02/skos/core#definition> "Accounting consolidation holds when \"[in the] financial statements of a group [...] the assets, liabilities, equity, income, expenses and cash flows of the parent and its subsidiaries are presented as those of a single economic entity (please see http://www.iasplus.com/en/standards/ias/ias27-2011)."@en .


###  http://lei.info/voc/l2/AccountingStandard
L2:AccountingStandard rdf:type owl:NamedIndividual ,
                               L2:RelationshipQualifierDimension ;
                      L2:level2CDFFName "ACCOUNTING_STANDARD"^^xsd:string ;
                      L2:level2CDFFType "rr:QualifierCategoryTypeEnum"^^xsd:string ;
                      rdfs:label "accounting standard"@en ;
                      <http://www.w3.org/2004/02/skos/core#definition> """The accounting standard applied to determine the definition of e.g. ultimate or direct accounting consolidating parent for the relationship detailed
in GLEIS RelationshipRecord. The relevant accounting standard is that applicable to the \"parent\" entity."""@en .


###  http://lei.info/voc/l2/AccountsFiling
L2:AccountsFiling rdf:type owl:NamedIndividual ,
                           L2:ValidationDocument ;
                  L2:level2CDFFName "ACCOUNTS_FILING"^^xsd:string ;
                  L2:level2CDFFType "ValidationDocumentsTypeEnum"^^xsd:string ;
                  rdfs:label "consolidated accounting statement"@en ;
                  <http://www.w3.org/2004/02/skos/core#definition> "A consolidated financial (accounting) statement, prepared and submitted to the relevant authority."@en .


###  http://lei.info/voc/l2/Active
L2:Active rdf:type owl:NamedIndividual ,
                   L2:RelationshipStatus ;
          L2:level2CDFFName "ACTIVE"^^xsd:string ;
          L2:level2CDFFType "rr:RelationshipStatusEnum"^^xsd:string ;
          rdfs:label "active"@en ;
          <http://www.w3.org/2004/02/skos/core#definition> "As of the last report or update, the reporting legal entity reported that it is legally registered and/or operating, AND that the relationship is still valid."@en .


###  http://lei.info/voc/l2/Annulled
L2:Annulled rdf:type owl:NamedIndividual ,
                     L2:RegistrationStatus ;
            L2:level2CDFFName "ANNULLED"^^xsd:string ;
            L2:level2CDFFType "rr:RegistrationStatusEnum"^^xsd:string ;
            rdfs:label "annulled"@en ;
            <http://www.w3.org/2004/02/skos/core#definition> "A relationship data report that was marked as erroneous or invalid after it was published. The relationship report is kept in publication for historical audit trail purposes only (so that data recipients can correct their local data)."@en .


###  http://lei.info/voc/l2/Contract
L2:Contract rdf:type owl:NamedIndividual ,
                     L2:ValidationDocument ;
            L2:level2CDFFName "CONTRACTS"^^xsd:string ;
            L2:level2CDFFType "ValidationDocumentsTypeEnum"^^xsd:string ;
            rdfs:label "Contact(s) attesting to the validity of the relationship"@en ;
            <http://www.w3.org/2004/02/skos/core#definition> "Contact(s) attesting to the validity of the relationship"@en .


###  http://lei.info/voc/l2/Duplicate
L2:Duplicate rdf:type owl:NamedIndividual ,
                      L2:RegistrationStatus ;
             L2:level2CDFFName "DUPLICATE"^^xsd:string ;
             L2:level2CDFFType "rr:RegistrationStatusEnum"^^xsd:string ;
             rdfs:label "duplicate"@en ;
             <http://www.w3.org/2004/02/skos/core#definition> "A relationship data report that has been determined to be a duplicate registration of the same relationship. In many cases this will mean more than one report with e.g. the same 2 entity IDs, the same relationship type, certain status values and the same relationship date(s), but this determination will depend on the relationship type in question."@en .


###  http://lei.info/voc/l2/EntitySuppliedOnly
L2:EntitySuppliedOnly rdf:type owl:NamedIndividual ,
                               L2:ValidationSource ;
                      L2:level2CDFFName "ENTITY_SUPPLIED_ONLY"^^xsd:string ;
                      L2:level2CDFFType "ValidationSourcesTypeEnum"^^xsd:string ;
                      rdfs:label "EntitySuppliedOnly"@en ;
                      <http://www.w3.org/2004/02/skos/core#definition> "Based on the validation procedures in use by the LOU responsible for the record, the information associated with this record has significant reliance on the information that a submitter provided due to the unavailability of corroborating information."@en .


###  http://lei.info/voc/l2/FullyCorroborated
L2:FullyCorroborated rdf:type owl:NamedIndividual ,
                              L2:ValidationSource ;
                     L2:level2CDFFName "FULLY_CORROBORATED"^^xsd:string ;
                     L2:level2CDFFType "ValidationSourcesTypeEnum"^^xsd:string ;
                     rdfs:label "fully corroborated"@en ;
                     <http://www.w3.org/2004/02/skos/core#definition> "The relationship data provided by the registrant has been validated against an explicit relationship statement found in key sources (e.g. consolidated financial statements)."@en .


###  http://lei.info/voc/l2/IFRS
L2:IFRS rdf:type owl:NamedIndividual ,
                 L2:RelationshipQualifierCategory ;
        L2:level2CDFFName "IFRS"^^xsd:string ;
        L2:level2CDFFType "rr:QualifierCategoryTypeEnum"^^xsd:string ;
        rdfs:label "International Financial Reporting Standard"@en ;
        <http://www.w3.org/2004/02/skos/core#definition> "International Financial Reporting Standard (developed by the International Accounting Standards Board  IASB see http://www.ifrs.org)."@en .


###  http://lei.info/voc/l2/Inactive
L2:Inactive rdf:type owl:NamedIndividual ,
                     L2:RelationshipStatus ;
            L2:level2CDFFName "INACTIVE"^^xsd:string ;
            L2:level2CDFFType "rr:RelationshipStatusEnum"^^xsd:string ;
            rdfs:label "inactive"@en ;
            <http://www.w3.org/2004/02/skos/core#definition> "It has been determined that the relationship ended, e.g. because entity that reported this relationship is no longer legally registered and/or operating; or the relationship is no longer valid for other reasons."@en .


###  http://lei.info/voc/l2/Lapsed
L2:Lapsed rdf:type owl:NamedIndividual ,
                   L2:RegistrationStatus ;
          L2:level2CDFFName "LAPSED"^^xsd:string ;
          L2:level2CDFFType "rr:RegistrationStatusEnum"^^xsd:string ;
          rdfs:label "lapsed"@en ;
          <http://www.w3.org/2004/02/skos/core#definition> "A relationship data report that has not been renewed by the next renewal date."@en .


###  http://lei.info/voc/l2/OtherAccountingStandard
L2:OtherAccountingStandard rdf:type owl:NamedIndividual ,
                                    L2:RelationshipQualifierCategory ;
                           L2:level2CDFFName "OTHER_ACCOUNTING_STANDARD"^^xsd:string ;
                           L2:level2CDFFType "rr:QualifierCategoryTypeEnum"^^xsd:string ;
                           rdfs:label "accounting standard different from IFRS and US_GAAP"@en ;
                           <http://www.w3.org/2004/02/skos/core#definition> "A financial reporting (accounting) standard not otherwise listed in the latest version of the relationship data file format."@en .


###  http://lei.info/voc/l2/PartiallyCorroborated
L2:PartiallyCorroborated rdf:type owl:NamedIndividual ,
                                  L2:ValidationSource ;
                         L2:level2CDFFName "PARTIALLY_CORROBORATED"^^xsd:string ;
                         L2:level2CDFFType "ValidationSourcesTypeEnum"^^xsd:string ;
                         rdfs:label "partially corroborated"@en ;
                         <http://www.w3.org/2004/02/skos/core#definition> "Based on the validation procedures in use by the LOU responsible for the record, the information supplied by the submitter can be partially corroborated by supporting sources (e.g. financial statements with other definitions of the relevant relationship type; quarterly or annual regulatory filings, contracts and other documents used in preparing financial statements)."@en .


###  http://lei.info/voc/l2/Pending
L2:Pending rdf:type owl:NamedIndividual ,
                    L2:ValidationSource ;
           L2:level2CDFFName "PENDING"^^xsd:string ;
           L2:level2CDFFType "ValidationSourcesTypeEnum"^^xsd:string ;
           rdfs:label "pending"@en ;
           <http://www.w3.org/2004/02/skos/core#definition> "The validation of the relationship data provided by the registrant has not yet occurred. Records with this validation sources value MUST not be published."@en .


###  http://lei.info/voc/l2/PendingArchival
L2:PendingArchival rdf:type owl:NamedIndividual ,
                            L2:RegistrationStatus ;
                   L2:level2CDFFName "PENDING_ARCHIVAL"^^xsd:string ;
                   L2:level2CDFFType "rr:RegistrationStatusEnum"^^xsd:string ;
                   rdfs:label "pending archival"@en ;
                   <http://www.w3.org/2004/02/skos/core#definition> "This relationship data report is about to be transferred to a different LOU, after which its registration status will revert to a non-pending status. The PendingArchival status serves to inform recipients of LOU-provided data files that a relationship record will be removed from that LOUs published file after the transfer is complete"@en .


###  http://lei.info/voc/l2/PendingTransfer
L2:PendingTransfer rdf:type owl:NamedIndividual ,
                            L2:RegistrationStatus ;
                   L2:level2CDFFName "PENDING_TRANSFER"^^xsd:string ;
                   L2:level2CDFFType "rr:RegistrationStatusEnum"^^xsd:string ;
                   rdfs:label "pending transfer"@en ;
                   <http://www.w3.org/2004/02/skos/core#definition> "A relationship data report for which a transfer to another LOU has been requested. The request is being processed at the sending LOU. When the receiving LOU is ready, the status will be changed to PendingArchival by the sending LOU prior to completion of the transfer."@en .


###  http://lei.info/voc/l2/PendingValidation
L2:PendingValidation rdf:type owl:NamedIndividual ,
                              L2:RegistrationStatus ;
                     L2:level2CDFFName "PENDING_VALIDATION"^^xsd:string ;
                     L2:level2CDFFType "rr:RegistrationStatusEnum"^^xsd:string ;
                     rdfs:label "pending validation"@en ;
                     <http://www.w3.org/2004/02/skos/core#definition> "A relationship data report that has been submitted to the LOU and which is being processed and validated, prior to publication."@en .


###  http://lei.info/voc/l2/Percentage
L2:Percentage rdf:type owl:NamedIndividual ,
                       L2:RelationshipQuantifierUnit ;
              L2:level2CDFFName "PERCENTAGE"^^xsd:string ;
              L2:level2CDFFType "QuantifierUnitsTypeEnum"^^xsd:string ;
              rdfs:label "percentage"@en .


###  http://lei.info/voc/l2/Published
L2:Published rdf:type owl:NamedIndividual ,
                      L2:RegistrationStatus ;
             L2:level2CDFFName "PUBLISHED"^^xsd:string ;
             L2:level2CDFFType "rr:RegistrationStatusEnum"^^xsd:string ;
             rdfs:label "published"@en ;
             <http://www.w3.org/2004/02/skos/core#definition> "A relationship data report that has been validated and published, and which is reported by an entity that was an operating legal entity as of the last update."@en .


###  http://lei.info/voc/l2/RegulatoryFiling
L2:RegulatoryFiling rdf:type owl:NamedIndividual ,
                             L2:ValidationDocument ;
                    L2:level2CDFFName "REGULATORY_FILING"^^xsd:string ;
                    L2:level2CDFFType "ValidationDocumentsTypeEnum"^^xsd:string ;
                    rdfs:label "annual regulatory filing"@en ;
                    <http://www.w3.org/2004/02/skos/core#definition> "An annual regulatory filing providing public information on parent relationships."@en .


###  http://lei.info/voc/l2/Retired
L2:Retired rdf:type owl:NamedIndividual ,
                    L2:RegistrationStatus ;
           L2:level2CDFFName "RETIRED"^^xsd:string ;
           L2:level2CDFFType "rr:RegistrationStatusEnum"^^xsd:string ;
           rdfs:label "retired"@en ;
           <http://www.w3.org/2004/02/skos/core#definition> "The relationship is considered to have ended, but the relationship report is kept in publication for historical audit trail purposes."@en .


###  http://lei.info/voc/l2/SupportingDocument
L2:SupportingDocument rdf:type owl:NamedIndividual ,
                               L2:ValidationDocument ;
                      L2:level2CDFFName "SUPPORTING_DOCUMENTS"^^xsd:string ;
                      L2:level2CDFFType "ValidationDocumentsTypeEnum"^^xsd:string ;
                      rdfs:label "Other documents supporting the preparation of consolidated financial statement"@en ;
                      <http://www.w3.org/2004/02/skos/core#definition> "Other documents supporting the preparation of consolidated financial statements"@en .


###  http://lei.info/voc/l2/Transferred
L2:Transferred rdf:type owl:NamedIndividual ,
                        L2:RegistrationStatus ;
               L2:level2CDFFName "TRANSFERRED"^^xsd:string ;
               L2:level2CDFFType "rr:RegistrationStatusEnum"^^xsd:string ;
               rdfs:label "transferred"@en ;
               <http://www.w3.org/2004/02/skos/core#definition> "A relationship data report that has been transferred to a different LOU as the managing LOU. A record in this state is not published, but may be used internally by the prior LOU for audit trail purposes."@en .


###  http://lei.info/voc/l2/USGAAP
L2:USGAAP rdf:type owl:NamedIndividual ,
                   L2:RelationshipQualifierCategory ;
          L2:level2CDFFName "US_GAAP"^^xsd:string ;
          L2:level2CDFFType "rr:QualifierCategoryTypeEnum"^^xsd:string ;
          rdfs:label "United States-Generally Accepted Accounting Principles"@en ;
          <http://www.w3.org/2004/02/skos/core#definition> "United States-Generally Accepted Accounting Principles."@en .


###  http://lei.info/voc/l2/isDirectlyConsolidatedBy
L2:isDirectlyConsolidatedBy rdf:type owl:NamedIndividual ,
                                     L2:RelationshipType ;
                            L2:level2CDFFName "IS_DIRECTLY_CONSOLIDATED_BY"^^xsd:string ;
                            L2:level2CDFFType "rr:RelationshipTypeEnum"^^xsd:string ;
                            rdfs:label "is directly consolidated by"@en ;
                            <http://www.w3.org/2004/02/skos/core#definition> "\"Child\" entity is directly consolidated by \"parent\" entity. The \"child\" entity has its accounts fully consolidated by the \"parent\" entity, in the sense given by the accounting standard(s) specified in RelationshipQualifier; the \"parent\" entity is the closest fully consolidating parent to the \"child\" entity in any applicable hierarchical ownership structure."@en .


###  http://lei.info/voc/l2/isInternationalBranchOf
L2:isInternationalBranchOf rdf:type owl:NamedIndividual ,
                                    L2:RelationshipType ;
                           L2:level2CDFFName "IS_INTERNATIONAL_BRANCH_OF"^^xsd:string ;
                           L2:level2CDFFType "rr:RelationshipTypeEnum"^^xsd:string ;
                           rdfs:label "is an international branch of"@en ;
                           <http://www.w3.org/2004/02/skos/core#definition> "\"Child\" entity is an international branch of the legal entity designated by \"parent\" entity  (in jurisdiction country of \"child\" entity). The \"parent\" entity is the Head Office and must have an LEI."@en .


###  http://lei.info/voc/l2/isUltimatelyConsolidatedBy
L2:isUltimatelyConsolidatedBy rdf:type owl:NamedIndividual ,
                                       L2:RelationshipType ;
                              L2:level2CDFFName "IS_ULTIMATELY_CONSOLIDATED_BY"^^xsd:string ;
                              L2:level2CDFFType "rr:RelationshipTypeEnum"^^xsd:string ;
                              rdfs:label "is ultimately consolidated by"@en ;
                              <http://www.w3.org/2004/02/skos/core#definition> "\"Child\" entity is ultimately consolidated by \"parent\" entity. The \"child\" entity has its accounts fully consolidated by the \"parent\" entity in the sense given by the accounting standard(s) specified in RelationshipQualifier; the \"parent\" entity is the most distant fully consolidating parent from the \"child\" entity in any applicable hierarchical ownership structure."@en .


###  http://lei.info/voc/l2/supplied
L2:supplied rdf:type owl:NamedIndividual ,
                     L2:ValidationDocument ;
            L2:level2CDFFName "OTHER_OFFICIAL_DOCUMENTS"^^xsd:string ;
            L2:level2CDFFType "ValidationDocumentsTypeEnum"^^xsd:string ;
            rdfs:label "Other official document(s) attesting to the validity of the relationship"@en ;
            <http://www.w3.org/2004/02/skos/core#definition> "Other official document(s) attesting to the validity of the relationship."@en .


[ owl:minQualifiedCardinality "0"^^xsd:nonNegativeInteger
] .

[ owl:qualifiedCardinality "1"^^xsd:nonNegativeInteger
 ] .

[ owl:qualifiedCardinality "1"^^xsd:nonNegativeInteger
 ] .

[ owl:qualifiedCardinality "1"^^xsd:nonNegativeInteger
 ] .

[ owl:qualifiedCardinality "1"^^xsd:nonNegativeInteger
 ] .

[ owl:qualifiedCardinality "1"^^xsd:nonNegativeInteger
 ] .

[ owl:maxQualifiedCardinality "1"^^xsd:nonNegativeInteger
 ] .

[ owl:qualifiedCardinality "1"^^xsd:nonNegativeInteger
 ] .

[ owl:qualifiedCardinality "1"^^xsd:nonNegativeInteger
 ] .

[ owl:qualifiedCardinality "1"^^xsd:nonNegativeInteger
 ] .

[ owl:qualifiedCardinality "1"^^xsd:nonNegativeInteger
 ] .

[ owl:qualifiedCardinality "1"^^xsd:nonNegativeInteger
 ] .

[ owl:qualifiedCardinality "1"^^xsd:nonNegativeInteger
 ] .

[ owl:qualifiedCardinality "1"^^xsd:nonNegativeInteger
 ] .

[ owl:qualifiedCardinality "1"^^xsd:nonNegativeInteger
 ] .

[ owl:minQualifiedCardinality "0"^^xsd:nonNegativeInteger
 ] .

[ owl:qualifiedCardinality "1"^^xsd:nonNegativeInteger
 ] .

[ owl:qualifiedCardinality "1"^^xsd:nonNegativeInteger
 ] .

[ owl:qualifiedCardinality "1"^^xsd:nonNegativeInteger
 ] .

[ owl:qualifiedCardinality "1"^^xsd:nonNegativeInteger
 ] .

[ owl:qualifiedCardinality "1"^^xsd:nonNegativeInteger
 ] .

#################################################################
#    General axioms
#################################################################

[ rdf:type owl:AllDisjointClasses ;
   owl:members ( L1:Address
                 L1:EntityCategory
                 L1:EntityExpirationReason
                 L1:EntityStatus
                 L1:LegalEntityIdentifier
                 L1:RegistrationAuthority
                 L1:RegistrationStatus
                 L1:ValidationAuthority
                 L1:ValidationSource
                 L2:MeasurementMethod
                 L2:RegistrationStatus
                 L2:Relationship
                 L2:RelationshipPeriodType
                 L2:RelationshipQualifier
                 L2:RelationshipQualifierCategory
                 L2:RelationshipQualifierDimension
                 L2:RelationshipQuantifier
                 L2:RelationshipQuantifierUnit
                 L2:RelationshipStatus
                 L2:RelationshipType
                 L2:ValidationDocument
                 L2:ValidationSource
               )
 ] .


[ rdf:type owl:AllDisjointClasses ;
  owl:members ( L2:AccountingPeriod
                L2:DocumentFilingPeriod
                L2:RelationshipPeriod
              )
] .


###  Generated by the OWL API (version 4.2.8.20170104-2310) https://github.com/owlcs/owlapi
